refactor until bfs_invar_init

BFS.thy
@@ -1,343 +1,2616 @@
 theory BFS
   imports
     "Graph_Theory/Graph_Theory"
-    Misc
     Queue_Specs
     Tbd
 begin
 
-record ('q, 'v) state =
+record ('q, 'a) state =
   queue :: 'q
-  distance :: "'v \<rightharpoonup> nat"
-  parent :: "'v \<rightharpoonup> 'v"
+  parent :: "'a \<rightharpoonup> 'a"
 
 locale bfs =
   finite_dgraph G +
-  (* tbd where fold = fold + *)
   Queue where snoc = snoc
   for
-    G :: "'v dgraph" and
-    (* fold :: "('v \<Rightarrow> ('q, 'v) state \<Rightarrow> ('q, 'v) state) \<Rightarrow> 'v set \<Rightarrow> ('q, 'v) state \<Rightarrow> ('q, 'v) state" and *)
-    snoc :: "'q \<Rightarrow> 'v \<Rightarrow> 'q" +
-  fixes src :: 'v
-  assumes src_in_V: "src \<in> dVs G"
+    G :: "'a::linorder dgraph" and
+    snoc :: "'q \<Rightarrow> 'a \<Rightarrow> 'q" +
+  fixes src :: 'a
+  assumes src_in_vertices: "src \<in> dVs G"
 
-section \<open>bfs Algorithm\<close>
+abbreviation (in bfs) dist :: "'a \<Rightarrow> enat" where
+  "dist \<equiv> Shortest_Dpath.dist G src"
 
-definition (in bfs) init :: "('q, 'v) state" where
-  "init \<equiv> \<lparr>queue = snoc empty src,
-           distance = [src \<mapsto> 0],
-           parent = [src \<mapsto> src]\<rparr>"
+section \<open>BFS Algorithm\<close>
 
-definition (in bfs) cond :: "('q, 'v) state \<Rightarrow> bool" where
+definition (in bfs) init :: "('q, 'a) state" where
+  "init \<equiv>
+   \<lparr>queue = snoc empty src,
+    parent = Map.empty\<rparr>"
+
+definition (in bfs) cond :: "('q, 'a) state \<Rightarrow> bool" where
   "cond s \<longleftrightarrow> \<not> is_empty (queue s)"
 
-definition (in bfs) discovered :: "'v \<Rightarrow> ('q, 'v) state \<Rightarrow> bool" where
-  "discovered v s \<longleftrightarrow> v \<in> dom (parent s)"
+definition (in bfs) discovered :: "('q, 'a) state \<Rightarrow> 'a \<Rightarrow> bool" where
+  "discovered s v \<longleftrightarrow> v = src \<or> v \<in> dom (parent s)"
 
-definition (in bfs) discover :: "'v \<Rightarrow> 'v \<Rightarrow> ('q, 'v) state \<Rightarrow> ('q, 'v) state" where
+definition (in bfs) discover :: "'a \<Rightarrow> 'a \<Rightarrow> ('q, 'a) state \<Rightarrow> ('q, 'a) state" where
   "discover u v s \<equiv>
-    if discovered v s then s
-    else
-      let
-        q = snoc (queue s) v;
-        d = distance s(v \<mapsto>
-          case distance s u of
-            Some n \<Rightarrow> Suc n);
-        p = parent s(v \<mapsto> u)
-      in \<lparr>queue = q, distance = d, parent = p\<rparr>"
+   \<lparr>queue = snoc (queue s) v,
+    parent = parent s(v \<mapsto> u)\<rparr>"
 
-function (in bfs) loop :: "('q, 'v) state \<Rightarrow> ('q, 'v) state" where
+definition (in bfs) traverse_edge :: "'a \<Rightarrow> 'a \<Rightarrow> ('q, 'a) state \<Rightarrow> ('q, 'a) state" where
+  "traverse_edge u v s \<equiv>
+   if \<not> discovered s v then discover u v s
+   else s"
+
+function (in bfs) (domintros) loop :: "('q, 'a) state \<Rightarrow> ('q, 'a) state" where
   "loop s =
-    (if cond s then
-       let
-        u = head (queue s);
-        q = tail (queue s)
-       in loop (Finite_Set.fold (discover u) (s\<lparr>queue := q\<rparr>) (out_neighborhood G u))
-     else s)"
+   (if cond s
+    then let
+          u = head (queue s);
+          q = tail (queue s)
+         in loop (fold (traverse_edge u) (sorted_list_of_set (out_neighborhood G u)) (s\<lparr>queue := q\<rparr>))
+    else s)"
   by pat_completeness simp
 
-definition (in bfs) bfs :: "('q, 'v) state" where
+abbreviation (in bfs) bfs :: "('q, 'a) state" where
   "bfs \<equiv> loop init"
+
+section \<open>\<close>
+
+abbreviation (in bfs) fold :: "('q, 'a) state \<Rightarrow> ('q, 'a) state" where
+  "fold s \<equiv>
+   List.fold
+    (traverse_edge (head (queue s)))
+    (sorted_list_of_set (out_neighborhood G (head (queue s))))
+    (s\<lparr>queue := tail (queue s)\<rparr>)"
+
+abbreviation (in bfs) T :: "('q, 'a) state \<Rightarrow> 'a dgraph" where
+  "T s \<equiv> {(u, v) |u v. parent s v = Some u}"
+
+section \<open>Convenience Lemmas\<close>
+
+subsection \<open>invar \<circ> queue\<close>
+
+lemma (in bfs) invar_tail:
+  assumes "invar (queue s)"
+  assumes "cond s"
+  shows "invar (queue (s\<lparr>queue := tail (queue s)\<rparr>))"
+  using assms invar_tail
+  by (simp add: cond_def is_empty)
+
+subsection \<open>list \<circ> queue\<close>
+
+lemma (in bfs) list_queue_non_empty:
+  assumes "invar (queue s)"
+  assumes "cond s"
+  shows "list (queue s) \<noteq> []"
+  using assms
+  by (simp add: cond_def is_empty)
+
+section \<open>Basic Lemmas\<close>
+
+subsection \<open>@{term bfs.discover}\<close>
+
+subsubsection \<open>queue\<close>
+
+lemma (in bfs) queue_discover_cong [simp]:
+  shows "queue (discover u v s) = snoc (queue s) v"
+  by (simp add: discover_def)
+
+subsubsection \<open>parent\<close>
+
+lemma (in bfs) parent_discover_cong [simp]:
+  shows "parent (discover u v s) = parent s ++ [v \<mapsto> u]"
+  by (simp add: discover_def)
+
+subsection \<open>@{term bfs.traverse_edge}\<close>
+
+subsubsection \<open>queue\<close>
+
+lemma (in bfs) queue_traverse_edge_cong:
+  shows "queue (traverse_edge u v s) = (if \<not> discovered s v then snoc (queue s) v else queue s)"
+  by (simp add: traverse_edge_def)
+
+subsubsection \<open>invar \<circ> queue\<close>
+
+lemma (in bfs) invar_queue_traverse_edge:
+  assumes "invar (queue s)"
+  shows "invar (queue (traverse_edge u v s))"
+  using assms invar_snoc
+  by (simp add: queue_traverse_edge_cong)
+
+subsubsection \<open>list \<circ> queue\<close>
+
+lemma (in bfs) list_queue_traverse_edge_cong:
+  assumes "invar (queue s)"
+  shows
+    "list (queue (traverse_edge u v s)) =
+     list (queue s) @ (if \<not> discovered s v then [v] else [])"
+  using assms
+  by (simp add: queue_traverse_edge_cong list_snoc)
+
+subsubsection \<open>parent\<close>
+
+lemma (in bfs) parent_traverse_edge_cong:
+  shows
+    "parent (traverse_edge u v s) =
+     parent s ++ (if \<not> discovered s v then [v \<mapsto> u] else Map.empty)"
+  by (simp add: traverse_edge_def)
+
+subsubsection \<open>@{term bfs.T}\<close>
+
+lemma (in bfs) T_traverse_edge_cong:
+  shows "T (traverse_edge u v s) = T s \<union> (if \<not> discovered s v then {(u, v)} else {})"
+  by (auto simp add: traverse_edge_def discovered_def discover_def)
+
+subsection \<open>@{term bfs.fold}\<close>
+
+subsubsection \<open>invar \<circ> queue\<close>
+
+lemma (in bfs) invar_queue_fold:
+  assumes "invar (queue s)"
+  assumes "distinct l"
+  shows "invar (queue (List.fold (traverse_edge u) l s))"
+  using assms
+  by (induct l arbitrary: s) (simp_all add: invar_queue_traverse_edge)
+
+lemma (in bfs) invar_queue_fold_2:
+  assumes "invar (queue s)"
+  assumes "cond s"
+  shows "invar (queue (fold s))"
+  using assms
+  by (auto intro: invar_tail invar_queue_fold)
+
+subsubsection \<open>list \<circ> queue\<close>
+
+lemma (in bfs) list_queue_fold_cong_aux:
+  assumes "distinct (v # vs)"
+  assumes "w \<in> set vs"
+  shows "discovered (traverse_edge u v s) w = discovered s w"
+  using assms
+  by (auto simp add: discovered_def parent_traverse_edge_cong)
+
+lemma (in bfs) list_queue_fold_cong:
+  assumes "invar (queue s)"
+  assumes "distinct l"
+  shows
+    "list (queue (List.fold (traverse_edge u) l s)) =
+     list (queue s) @ filter (Not \<circ> discovered s) l"
+  using assms
+proof (induct l arbitrary: s)
+  case Nil
+  thus ?case
+    by simp
+next
+  case (Cons v vs)    
+  have
+    "list (queue (List.fold (traverse_edge u) (v # vs) s)) =
+     list (queue (List.fold (traverse_edge u) vs (traverse_edge u v s)))"
+    by simp
+  also have
+    "... =
+     list (queue (traverse_edge u v s)) @
+     filter (Not \<circ> discovered (traverse_edge u v s)) vs"
+    using Cons.prems
+    by (auto intro: invar_queue_traverse_edge Cons.hyps)
+  also have
+    "... =
+     list (queue s) @
+     (if \<not> discovered s v then [v] else []) @
+     filter (Not \<circ> discovered (traverse_edge u v s)) vs"
+    using Cons.prems(1)
+    by (simp add: list_queue_traverse_edge_cong)
+  also have
+    "... =
+     list (queue s) @
+     (if \<not> discovered s v then [v] else []) @
+     filter (Not \<circ> discovered s) vs"
+    unfolding comp_apply
+    using Cons.prems(2)
+    by (auto simp add: list_queue_fold_cong_aux intro: filter_cong)
+  also have "... = list (queue s) @ filter (Not \<circ> discovered s) (v # vs)"
+    by simp
+  finally show ?case
+    .
+qed
+
+lemma (in bfs) list_queue_fold_cong_2:
+  assumes "invar (queue s)"
+  assumes "cond s"
+  shows
+    "list (queue (fold s)) =
+     list (tail (queue s)) @
+     filter (Not \<circ> discovered s) (sorted_list_of_set (out_neighborhood G (head (queue s))))"
+proof -
+  have
+    "list (queue (fold s)) =
+     list (queue (s\<lparr>queue := tail (queue s)\<rparr>)) @
+     filter
+      (Not \<circ> discovered (s\<lparr>queue := tail (queue s)\<rparr>))
+      (sorted_list_of_set (out_neighborhood G (head (queue s))))"
+    using assms
+    by (intro invar_tail list_queue_fold_cong) simp+
+  also have
+    "... =
+     list (tail (queue s)) @
+     filter
+      (Not \<circ> discovered s)
+      (sorted_list_of_set (out_neighborhood G (head (queue s))))"
+    unfolding comp_apply
+    by (simp add: discovered_def)
+  finally show ?thesis
+    .
+qed
+
+subsubsection \<open>parent\<close>
+
+lemma (in bfs) parent_fold_cong_aux:
+  assumes "distinct (v # vs)"
+  shows "w \<in> set vs \<and> \<not> discovered (traverse_edge u v s) w \<longleftrightarrow> w \<in> set vs \<and> \<not> discovered s w"
+  using assms
+  by (auto simp add: discovered_def parent_traverse_edge_cong)
+
+lemma (in bfs) parent_fold_cong:
+  assumes "distinct l"
+  shows
+    "parent (List.fold (traverse_edge u) l s) =
+     parent s ++ (\<lambda>v. if v \<in> set l \<and> \<not> discovered s v then Some u else None)"
+  using assms
+proof (induct l arbitrary: s)
+  case Nil
+  thus ?case
+    by simp
+next
+  case (Cons v vs)
+  have
+    "parent (List.fold (traverse_edge u) (v # vs) s) =
+     parent (List.fold (traverse_edge u) vs (traverse_edge u v s))"
+    by simp
+  also have
+    "... =
+     parent (traverse_edge u v s) ++
+     (\<lambda>w. if w \<in> set vs \<and> \<not> discovered (traverse_edge u v s) w then Some u else None)"
+    using Cons.prems
+    by (intro Cons.hyps) simp
+  also have
+    "... =
+     parent s ++
+     (if \<not> discovered s v then [v \<mapsto> u] else Map.empty) ++
+     (\<lambda>w. if w \<in> set vs \<and> \<not> discovered (traverse_edge u v s) w then Some u else None)"
+    by (simp add: parent_traverse_edge_cong)
+  also have
+    "... =
+     parent s ++
+     (if \<not> discovered s v then [v \<mapsto> u] else Map.empty) ++
+     (\<lambda>w. if w \<in> set vs \<and> \<not> discovered s w then Some u else None)"
+    using Cons.prems
+    by (simp add: parent_fold_cong_aux)
+  also have
+    "... =
+     parent s ++
+     (\<lambda>w. if w \<in> set (v # vs) \<and> \<not> discovered s w then Some u else None)"
+    using Cons.prems
+    by (auto simp add: map_add_def)
+  finally show ?case
+    .
+qed
+
+lemma (in bfs) parent_fold_cong_2:
+  shows
+    "parent (fold s) =
+     parent s ++
+     (\<lambda>v. if v \<in> set (sorted_list_of_set (out_neighborhood G (head (queue s)))) \<and> \<not> discovered s v
+          then Some (head (queue s))
+          else None)"
+proof -
+  have
+    "parent (fold s) =
+     parent (s\<lparr>queue := tail (queue s)\<rparr>) ++
+     (\<lambda>v. if v \<in> set (sorted_list_of_set (out_neighborhood G (head (queue s)))) \<and>
+             \<not> discovered (s\<lparr>queue := tail (queue s)\<rparr>) v
+          then Some (head (queue s))
+          else None)"
+    by (simp add: parent_fold_cong)
+  thus ?thesis
+    by (simp add: discovered_def)
+qed
+
+(* TODO: remove? *)
+lemma (in bfs) parent_le_parent_fold:
+  shows "parent s \<subseteq>\<^sub>m parent (fold s)"
+  unfolding map_le_def
+proof
+  fix v
+  assume "v \<in> dom (parent s)"
+  hence "discovered s v"
+    by (simp add: discovered_def)
+  thus "parent s v = parent (fold s) v"
+    by (simp add: parent_fold_cong_2 map_add_def)
+qed
+
+subsubsection \<open>dom \<circ> parent\<close>
+
+lemma (in bfs) dom_parent_fold_subset_vertices:
+  assumes "dom (parent s) \<subseteq> dVs G"
+  assumes "distinct l"
+  assumes "set l \<subseteq> dVs G"
+  shows "dom (parent (List.fold (traverse_edge u) l s)) \<subseteq> dVs G"
+  using assms
+  by (auto simp add: parent_fold_cong split: if_splits(2))
+
+lemma (in bfs) dom_parent_fold_subset_vertices_2:
+  assumes "dom (parent s) \<subseteq> dVs G"
+  shows "dom (parent (fold s)) \<subseteq> dVs G"
+proof -
+  have "set (sorted_list_of_set (out_neighborhood G (head (queue s)))) \<subseteq> dVs G"
+    using out_neighborhood_finite out_neighborhood_subset_vertices
+    by simp
+  thus ?thesis
+    using assms dom_parent_fold_subset_vertices
+    by simp
+qed
+
+subsubsection \<open>@{term bfs.T}\<close>
+
+lemma (in bfs) T_fold_cong:
+  assumes "distinct l"
+  shows "T (List.fold (traverse_edge u) l s) = T s \<union> {(u, v) |v. v \<in> set l \<and> \<not> discovered s v}"
+  using assms
+proof (induct l arbitrary: s)
+  case Nil
+  thus ?case
+    by auto
+next
+  case (Cons v vs)
+  have
+    "T (List.fold (traverse_edge u) (v # vs) s) =
+     T (List.fold (traverse_edge u) vs (traverse_edge u v s))"
+    by simp
+  also have
+    "... =
+     T (traverse_edge u v s) \<union>
+     {(u, w) |w. w \<in> set vs \<and> \<not> discovered (traverse_edge u v s) w}"
+    using Cons.prems
+    by (intro Cons.hyps) simp
+  also have
+    "... =
+     T s \<union>
+     (if \<not> discovered s v then {(u, v)} else {}) \<union>
+     {(u, w) |w. w \<in> set vs \<and> \<not> discovered (traverse_edge u v s) w}"
+    unfolding T_traverse_edge_cong
+    by blast
+  also have
+    "... =
+     T s \<union>
+     (if \<not> discovered s v then {(u, v)} else {}) \<union>
+     {(u, w) |w. w \<in> set vs \<and> \<not> discovered s w}"
+    using Cons.prems
+    by (simp add: parent_fold_cong_aux)
+  also have "... = T s \<union> {(u, w) |w. w \<in> set (v # vs) \<and> \<not> discovered s w}"
+    by force
+  finally show ?case
+    .
+qed
+
+lemma (in bfs) T_fold_cong_2:
+  shows
+    "T (fold s) =
+     T s \<union>
+     {(head (queue s), v) |v.
+      v \<in> set (sorted_list_of_set (out_neighborhood G (head (queue s)))) \<and> \<not> discovered s v}"
+proof -
+  have
+    "T (fold s) =
+     T (s\<lparr>queue := tail (queue s)\<rparr>) \<union>
+     {(head (queue s), v) |v.
+      v \<in> set (sorted_list_of_set (out_neighborhood G (head (queue s)))) \<and>
+      \<not> discovered (s\<lparr>queue := tail (queue s)\<rparr>) v}"
+    by (intro T_fold_cong) simp
+  thus ?thesis
+    by (simp add: discovered_def)
+qed
+
+section \<open>Termination\<close>
+
+lemma (in bfs) loop_dom_aux:
+  assumes "dom (parent s) \<subseteq> dVs G"
+  shows
+    "card (dom (parent (fold s))) =
+     card (dom (parent s)) +
+     card {v \<in> set (sorted_list_of_set (out_neighborhood G (head (queue s)))). \<not> discovered s v}"
+proof -
+  let ?S = "{v \<in> set (sorted_list_of_set (out_neighborhood G (head (queue s)))). \<not> discovered s v}"
+  have "dom (parent (fold s)) = dom (parent s) \<union> ?S"
+    by (auto simp add: parent_fold_cong_2 domIff)
+  moreover have "finite (dom (parent s))"
+    using assms vertices_finite
+    by (rule finite_subset)
+  moreover have "finite ?S"
+    using out_neighborhood_finite
+    by simp
+  moreover have "dom (parent s) \<inter> ?S = {}"
+    by (auto simp add: discovered_def)
+  ultimately show ?thesis
+    by (simp add: card_Un_disjoint)
+qed
+
+lemma (in bfs) loop_dom_aux_2:
+  assumes invar_queue: "invar (queue s)"
+  assumes cond: "cond s"
+  assumes dom_parent_subset_vertices: "dom (parent s) \<subseteq> dVs G"
+  shows
+    "card (dVs G) +
+     length (list (tail (queue s))) -
+     card (dom (parent s)) <
+     card (dVs G) +
+     length (list (queue s)) -
+     card (dom (parent s))"
+proof -
+  have "list (queue s) \<noteq> []"
+    using invar_queue cond
+    by (intro list_queue_non_empty)
+  hence "length (list (tail (queue s))) < length (list (queue s))"
+    using invar_queue
+    by (simp add: list_tail)
+  moreover have "card (dom (parent s)) \<le> card (dVs G)"
+    using vertices_finite dom_parent_subset_vertices
+    by (intro card_mono)
+  ultimately show ?thesis
+    by simp
+qed
+
+lemma (in bfs) loop_dom:
+  assumes "invar (queue s)"
+  assumes "dom (parent s) \<subseteq> dVs G"
+  shows "loop_dom s"
+  using assms
+proof (induct "card (dVs G) + length (list (queue s)) - card (dom (parent s))"
+       arbitrary: s
+       rule: less_induct)
+  case less
+  show ?case
+  proof (cases "cond s")
+    case True
+    let ?u = "head (queue s)"
+    let ?q = "tail (queue s)"
+    let ?S = "{v \<in> set (sorted_list_of_set (out_neighborhood G ?u)). \<not> discovered s v}"
+
+    have "length (list (queue (fold s))) = length (list ?q) + card ?S"
+      using less.prems(1) True
+      by (simp add: list_queue_fold_cong_2 distinct_card[symmetric])
+    moreover have "card (dom (parent (fold s))) = card (dom (parent s)) + card ?S"
+      using less.prems(2)
+      by (intro loop_dom_aux)
+    ultimately have
+      "card (dVs G) + length (list (queue (fold s))) - card (dom (parent (fold s))) =
+       card (dVs G) + length (list ?q) + card ?S - (card (dom (parent s)) + card ?S)"
+      by presburger
+    also have "... = card (dVs G) + length (list ?q) - card (dom (parent s))"
+      by simp
+    also have "... < card (dVs G) + length (list (queue s)) - card (dom (parent s))"
+      using less.prems True
+      by (intro loop_dom_aux_2)
+    finally have
+      "card (dVs G) + length (list (queue (fold s))) - card (dom (parent (fold s))) <
+       card (dVs G) + length (list (queue s)) - card (dom (parent s))"
+      .
+    thus ?thesis
+      using less.prems
+      by (intro invar_queue_fold_2 dom_parent_fold_subset_vertices_2 less.hyps loop.domintros)
+  next
+    case False
+    thus ?thesis
+      by (blast intro: loop.domintros)
+  qed
+qed
 
 section \<open>Invariants\<close>
 
-locale bfs_invar = bfs where G = G and (* fold = fold and *) snoc = snoc
+subsection \<open>\<close>
+
+abbreviation (in bfs) white :: "('q, 'a) state \<Rightarrow> 'a \<Rightarrow> bool" where
+  "white s v \<equiv> \<not> discovered s v"
+
+abbreviation (in bfs) gray :: "('q, 'a) state \<Rightarrow> 'a \<Rightarrow> bool" where
+  "gray s v \<equiv> discovered s v \<and> v \<in> set (list (queue s))"
+
+lemma (in bfs) gray_imp_not_white:
+  assumes "gray s v"
+  shows "\<not> white s v"
+  using assms
+  by simp
+
+abbreviation (in bfs) black :: "('q, 'a) state \<Rightarrow> 'a \<Rightarrow> bool" where
+  "black s v \<equiv> discovered s v \<and> v \<notin> set (list (queue s))"
+
+lemma (in bfs) black_imp_not_white:
+  assumes "black s v"
+  shows "\<not> white s v"
+  using assms
+  by simp
+
+lemma (in bfs) vertex_color_induct [case_names white gray black]:
+  assumes "white s v \<Longrightarrow> P s v"
+  assumes "gray s v \<Longrightarrow> P s v"
+  assumes "black s v \<Longrightarrow> P s v"
+  shows "P s v"
+  using assms
+  by blast
+
+locale bfs_invar =
+  bfs where G = G and snoc = snoc +
+  parent "state.parent s"
   for
-    G :: "'v dgraph" and
-    (* fold :: "('v \<Rightarrow> ('q, 'v) state \<Rightarrow> ('q, 'v) state) \<Rightarrow> 'v set \<Rightarrow> ('q, 'v) state \<Rightarrow> ('q, 'v) state" and *)
-    snoc :: "'q \<Rightarrow> 'v \<Rightarrow> 'q" +
-  fixes s :: "('q, 'v) state"
-  assumes queue_subset_V: "set (list (queue s)) \<subseteq> dVs G"
+    G :: "'a::linorder dgraph" and
+    snoc :: "'q \<Rightarrow> 'a \<Rightarrow> 'q" and
+    s :: "('q, 'a) state" +
+  assumes invar_queue: "invar (queue s)"
+  assumes queue_distinct: "distinct (list (queue s))"
+  assumes parent_src: "parent s src = None"
+  assumes gray_if_mem_queue: "v \<in> set (list (queue s)) \<Longrightarrow> gray s v"
+  assumes black_if_mem_ran: "v \<in> ran (parent s) \<Longrightarrow> black s v"
+  assumes queue_sorted_wrt_dpath_length:
+    "\<not> is_empty (queue s) \<Longrightarrow>
+     sorted_wrt (\<lambda>u v. dpath_length (rev (follow u)) \<le> dpath_length (rev (follow v))) (list (queue s)) \<and>
+     dpath_length (rev (follow (last (list (queue s))))) \<le> dpath_length (rev (follow (head (queue s)))) + 1"
+  assumes not_white_imp_shortest_dpath:
+    "\<not> white s v \<Longrightarrow> dpath_bet G (rev (follow v)) src v \<and> dpath_length (rev (follow v)) = dist v"
+  assumes black_imp_out_neighborhood_not_white: "black s v \<Longrightarrow> \<forall>w\<in>out_neighborhood G v. \<not> white s w"
+
+subsection \<open>Convenience Lemmas\<close>
+
+lemma (in bfs_invar) src_not_white:
+  shows "\<not> white s src"
+  by (simp add: discovered_def)
+
+(* TODO: move somewhere else *)
+lemma sorted_wrt_imp_hd:
+  assumes l_sorted_wrt: "sorted_wrt P l"
+  assumes x_mem_l: "x \<in> set l"
+  assumes x_not_hd: "x \<noteq> hd l"
+  shows "P (hd l) x"
+proof -
+  have "l \<noteq> []"
+    using x_mem_l
+    by fastforce
+  hence hd_eq_0th: "hd l = l ! 0"
+    by (simp add: hd_conv_nth)
+  obtain i where
+    "i < length l" and
+    x_eq_ith: "x = l ! i"
+    using x_mem_l
+    by (auto simp add: in_set_conv_nth)
+  moreover have "0 < i"
+    using x_not_hd
+    by (auto simp add: hd_eq_0th x_eq_ith intro: gr0I)
+  ultimately show ?thesis
+    using l_sorted_wrt
+    by (auto simp add: hd_eq_0th x_eq_ith intro: sorted_wrt_nth_less)
+qed
+
+lemma (in bfs_invar) mem_queue_imp_dpath_length_head_queue:
+  assumes "v \<in> set (list (queue s))"
+  shows "dpath_length (rev (follow (head (queue s)))) \<le> dpath_length (rev (follow v))"
+proof (cases "v = head (queue s)")
+  case True
+  thus ?thesis
+    by simp
+next
+  case False
+  have "\<not> is_empty (queue s)"
+    using invar_queue assms
+    by (auto simp add: is_empty)
+  moreover hence "head (queue s) = hd (list (queue s))"
+    using invar_queue list_head
+    by (simp add: is_empty)
+  ultimately show ?thesis
+    using queue_sorted_wrt_dpath_length assms False sorted_wrt_imp_hd
+    by fastforce
+qed
+
+lemma (in bfs_invar) mem_queue_imp_dist_head_queue:
+  assumes "v \<in> set (list (queue s))"
+  shows "dist (head (queue s)) \<le> dist v"
+proof -
+  have "list (queue s) \<noteq> []"
+    using assms
+    by fastforce
+  hence "head (queue s) \<in> set (list (queue s))"
+    using invar_queue
+    by (simp add: list_head)
+  hence "dist (head (queue s)) = dpath_length (rev (follow (head (queue s))))"
+    using gray_if_mem_queue
+    by (simp add: not_white_imp_shortest_dpath)
+  also have "... \<le> dpath_length (rev (follow v))"
+    using assms
+    by (auto intro: mem_queue_imp_dpath_length_head_queue)
+  also have "... = dist v"
+    using assms gray_if_mem_queue
+    by (simp add: not_white_imp_shortest_dpath)
+  finally show ?thesis
+    .
+qed
+
+(* TODO: move somewhere else *)
+lemma sorted_wrt_imp_last_aux:
+  assumes x_mem_l: "x \<in> set l"
+  assumes x_neq_last: "x \<noteq> last l"
+  obtains i where
+    "i < length l - 1"
+    "x = l ! i"
+proof -
+  have l_non_empty: "l \<noteq> []"
+    using x_mem_l
+    by fastforce
+  obtain i where
+    "i < length l" and
+    x_eq_ith: "x = l ! i"
+    using x_mem_l
+    by (auto simp add: in_set_conv_nth)
+  hence "i < Suc (length l - 1)"
+    by simp
+  moreover have "i \<noteq> length l - 1"
+    using x_neq_last l_non_empty
+    by (auto simp add: x_eq_ith last_conv_nth)
+  ultimately have "i < length l - 1"
+    by (elim less_SucE) simp+
+  thus ?thesis
+    using x_eq_ith
+    by (intro that)
+qed
+
+(* TODO: move somewhere else *)
+lemma sorted_wrt_imp_last:
+  assumes l_sorted_wrt: "sorted_wrt P l"
+  assumes x_mem_l: "x \<in> set l"
+  assumes x_neq_last: "x \<noteq> last l"
+  shows "P x (last l)"
+proof -
+  have "l \<noteq> []"
+    using x_mem_l
+    by fastforce
+  hence last_eq: "last l = l ! (length l - 1)"
+    by (simp add: last_conv_nth)
+  obtain i where
+    "i < length l - 1" and
+    x_eq_ith: "x = l ! i"
+    using assms(2, 3)
+    by (elim sorted_wrt_imp_last_aux)
+  thus ?thesis
+    using l_sorted_wrt
+    by (auto simp add: x_eq_ith last_eq intro: sorted_wrt_nth_less)
+qed
+
+lemma (in bfs_invar) mem_queue_imp_dpath_length_last_queue:
+  assumes "v \<in> set (list (queue s))"
+  shows "dpath_length (rev (follow v)) \<le> dpath_length (rev (follow (last (list (queue s)))))"
+proof (cases "v = last (list (queue s))")
+  case True
+  thus ?thesis
+    by simp
+next
+  case False
+  have "\<not> is_empty (queue s)"
+    using invar_queue assms
+    by (auto simp add: is_empty)
+  thus ?thesis
+    using queue_sorted_wrt_dpath_length assms False sorted_wrt_imp_last
+    by fastforce
+qed
+
+lemma (in bfs_invar) mem_queue_imp_dist_last_queue:
+  assumes "v \<in> set (list (queue s))"
+  shows "dist v \<le> dist (last (list (queue s)))"
+proof -
+  have list_queue_non_empty: "list (queue s) \<noteq> []"
+    using assms
+    by fastforce
+  have "dist v = dpath_length (rev (follow v))"
+    using assms gray_if_mem_queue
+    by (simp add: not_white_imp_shortest_dpath)
+  also have "... \<le> dpath_length (rev (follow (last (list (queue s)))))"
+    using assms
+    by (auto intro: mem_queue_imp_dpath_length_last_queue)
+  also have "... = dist (last (list (queue s)))"
+    using list_queue_non_empty gray_if_mem_queue
+    by (simp add: not_white_imp_shortest_dpath)
+  finally show ?thesis
+    .
+qed
+
+lemma (in bfs_invar) mem_queue_dpath_lengthI:
+  assumes "v \<in> set (list (queue s))"
+  shows
+    "dpath_length (rev (follow (head (queue s)))) \<le> dpath_length (rev (follow v))"
+    "dpath_length (rev (follow v)) \<le> dpath_length (rev (follow (last (list (queue s)))))"
+  using assms
+  by (auto intro: mem_queue_imp_dpath_length_head_queue mem_queue_imp_dpath_length_last_queue)
+
+lemma (in bfs_invar) mem_queue_distI:
+  assumes "v \<in> set (list (queue s))"
+  shows
+    "dist (head (queue s)) \<le> dist v"
+    "dist v \<le> dist (last (list (queue s)))"
+  using assms
+  by (auto intro: mem_queue_imp_dist_head_queue mem_queue_imp_dist_last_queue)
+
+subsection \<open>Basic Lemmas\<close>
+
+lemma (in bfs_invar) parent_imp_edge:
+  assumes "parent s v = Some u"
+  shows "(u, v) \<in> G"
+proof -
+  have "rev (follow v) = rev (follow u) @ [v]"
+    using assms
+    by (simp add: follow_psimps)
+  moreover have "rev (follow u) = (rev (tl (follow u))) @ [u]"
+    using follow_non_empty hd_Cons_tl follow_ConsD rev.simps(2)
+    by metis
+  ultimately have "rev (follow v) = rev (tl (follow u)) @ [u, v]"
+    by simp
+  moreover have "dpath_bet G (rev (follow v)) src v"
+    using assms not_white_imp_shortest_dpath
+    by (simp add: discovered_def domIff)
+  ultimately have "dpath_bet G (rev (tl (follow u)) @ [u, v]) src v"
+    by simp
+  thus ?thesis
+    by (auto simp add: edge_iff_dpath_bet intro: split_dpath)
+qed
+
+lemma (in bfs_invar) dom_parent_subset_vertices:
+  shows "dom (parent s) \<subseteq> dVs G"
+proof
+  fix v
+  assume "v \<in> dom (parent s)"
+  then obtain u where
+    "parent s v = Some u"
+    by (auto simp add: domIff)
+  hence "(u, v) \<in> G"
+    by (intro parent_imp_edge)
+  thus "v \<in> dVs G"
+    by (intro dVsI(2))
+qed
+
+lemma (in bfs_invar) queue_sorted_wrt_dist:
+  assumes "\<not> is_empty (queue s)"
+  shows
+    "sorted_wrt (\<lambda>u v. dist u \<le> dist v) (list (queue s))"
+    "dist (last (list (queue s))) \<le> dist (head (queue s)) + 1"
+proof -
+  have dpath_length_follow_eq_dist: "\<forall>v\<in>set (list (queue s)). dpath_length (rev (follow v)) = dist v"
+    using gray_if_mem_queue not_white_imp_shortest_dpath
+    by blast
+  hence
+    "\<And>u v. u \<in> set (list (queue s)) \<Longrightarrow>
+            v \<in> set (list (queue s)) \<Longrightarrow>
+            dpath_length (rev (follow u)) \<le> dpath_length (rev (follow v)) \<Longrightarrow>
+            (\<lambda>u v. dist u \<le> dist v) u v"
+    using assms
+    by (simp add: enat_ord_simps(1)[symmetric])
+  thus "sorted_wrt (\<lambda>u v. dist u \<le> dist v) (list (queue s))"
+    using assms queue_sorted_wrt_dpath_length sorted_wrt_mono_rel[of "(list (queue s))"]
+    by presburger
+  have
+    "last (list (queue s)) \<in> set (list (queue s))"
+    "head (queue s) \<in> set (list (queue s))"
+    using invar_queue assms
+    by (simp_all add: is_empty list_head)
+  thus "dist (last (list (queue s))) \<le> dist (head (queue s)) + 1"
+    using assms queue_sorted_wrt_dpath_length dpath_length_follow_eq_dist
+    unfolding enat_ord_simps(1)[symmetric] plus_enat_simps(1)[symmetric] one_enat_def[symmetric]
+    by simp
+qed
+
+lemma (in bfs_invar) white_imp_gray_ancestor:
+  assumes "dpath_bet G p u v"
+  assumes "\<not> white s u"
+  assumes "white s v"
+  shows "\<exists>v\<in>set p. gray s v"
+  using assms
+proof (induct p arbitrary: v rule: dpath_rev_induct)
+  case 1
+  thus ?case
+    by simp
+next
+  case (2 w)
+  hence "[w] = [u] \<and> u = v"
+    by (intro hd_of_dpath_bet' last_of_dpath_bet list_length_1) simp
+  thus ?case
+    using "2.prems"(2, 3)
+    by simp
+next
+  case (3 w w' l)
+  show ?case
+  proof (induct s w rule: vertex_color_induct)
+    case white
+    have "dpath_bet G (l @ [w]) u w"
+      using "3.prems"(1)
+      by (intro dpath_bet_pref) simp
+    hence "\<exists>v\<in>set (l @ [w]). gray s v"
+      using "3.prems"(2) white
+      by (intro "3.hyps")
+    thus ?thesis
+      by auto
+  next
+    case gray
+    thus ?thesis
+      by simp
+  next
+    case black
+    have "v \<in> out_neighborhood G w"
+      using "3.prems"(1)
+      by (auto simp add: dpath_bet_def in_out_neighborhood_iff_edge intro: dpath_snoc_edge_2)
+    hence "\<not> white s v"
+      using black black_imp_out_neighborhood_not_white
+        by blast
+    thus ?thesis
+      using "3.prems"(3)
+      by simp
+  qed
+qed
+
+lemma (in bfs_invar) white_imp_dist_ge_case_1_subcase_3:
+  assumes IH:
+    "\<And>v. \<lbrakk> dpath_bet G (l @ [u]) src v \<and> dpath_length (l @ [u]) = dist v; white s v \<rbrakk> \<Longrightarrow>
+          (if is_empty (queue s) then \<infinity> else dist (last (list (queue s)))) \<le> dist v"
+  assumes shortest_dpath: "dpath_bet G (l @ [u, u']) src v \<and> dpath_length (l @ [u, u']) = dist v"
+  assumes white: "white s v"
+  shows "(if is_empty (queue s) then \<infinity> else dist (last (list (queue s)))) \<le> dist v"
+proof (induct s u rule: vertex_color_induct)
+  case white
+  have l_snoc_u_shortest_dpath: "dpath_bet G (l @ [u]) src u \<and> dpath_length (l @ [u]) = dist u"
+    using shortest_dpath
+    by
+      (auto
+       simp add: dpath_length_eq_dpath_weight dist_eq_\<delta> is_shortest_dpath_def[symmetric]
+       intro: shortest_dpath_prefix_is_shortest_dpath)
+  hence "(if is_empty (queue s) then \<infinity> else dist (last (list (queue s)))) \<le> dist u"
+    using white
+    by (intro IH)
+  also have "... = dpath_length (l @ [u])"
+    by (simp add: l_snoc_u_shortest_dpath)
+  also have "... \<le> dpath_length (l @ [u, u'])"
+    using dpath_length_append[where ?p = "l @ [u]" and ?q = "[u']"]
+    by simp
+  also have "... = dist v"
+    by (simp add: shortest_dpath)
+  finally show ?case
+    .
+next
+  case gray
+  hence "\<exists>v\<in>set (l @ [u, u']). gray s v"
+    using src_not_white shortest_dpath white
+    by (blast intro: white_imp_gray_ancestor)
+  hence queue_non_empty: "\<not> is_empty (queue s)"
+    using invar_queue
+    by (auto simp add: is_empty)
+  hence "dist (last (list (queue s))) \<le> dist (head (queue s)) + 1"
+    by (intro queue_sorted_wrt_dist(2))
+  also have "... \<le> dist u + 1"
+    using gray
+    by (blast intro: mem_queue_imp_dist_head_queue add_right_mono)
+  also have "... = dist v"
+    using shortest_dpath
+    by (auto intro: shortest_dpathE_2)
+  finally show ?case
+    using queue_non_empty
+    by simp
+next
+  case black
+  have "v \<in> out_neighborhood G u"
+    using shortest_dpath last_of_dpath_bet
+    by (fastforce simp add: edge_iff_dpath_bet in_out_neighborhood_iff_edge intro: split_dpath)
+  hence "\<not> white s v"
+    using black black_imp_out_neighborhood_not_white
+    by blast
+  thus ?case
+    using white
+    by simp
+qed
+
+lemma (in bfs_invar) white_imp_dist_ge_case_1:
+  assumes "dpath_bet G p src v \<and> dpath_length p = dist v"
+  assumes "white s v"
+  shows "(if is_empty (queue s) then \<infinity> else dist (last (list (queue s)))) \<le> dist v"
+  using assms
+proof (induct p arbitrary: v rule: dpath_rev_induct)
+  case 1
+  thus ?case
+    by simp
+next
+  case (2 u)
+  hence "[u] = [src] \<and> src = v"
+    by (intro hd_of_dpath_bet' last_of_dpath_bet list_length_1) auto
+  thus ?case
+    using src_not_white "2.prems"(2)
+    by simp
+next
+  case (3 u u' l)
+  thus ?case
+    by (rule white_imp_dist_ge_case_1_subcase_3)
+qed
+
+lemma (in bfs_invar) white_imp_dist_ge:
+  assumes "white s v"
+  shows "(if is_empty (queue s) then \<infinity> else dist (last (list (queue s)))) \<le> dist v"
+proof (cases "reachable G src v")
+  case True
+  then obtain p where
+    "dpath_bet G p src v \<and> dpath_length p = dist v"
+    by (elim dist_dpath_betE) simp
+  thus ?thesis
+    using assms
+    by (intro white_imp_dist_ge_case_1)
+next
+  case False
+  hence "dist v = \<infinity>"
+    unfolding dist_eq_\<delta>
+    by (meson \<delta>_reachable_conv)
+  thus ?thesis
+    by simp
+qed
+
+subsection \<open>@{term bfs.init}\<close>
+
+subsubsection \<open>\<close>
+
+lemma (in bfs) follow_invar'_parent_init:
+  shows "follow_invar' (parent init)"
+  using wf_empty
+  by (simp add: follow_invar'_def init_def)
+
+lemma (in bfs) parent_init:
+  shows "Tbd.parent (parent init)"
+  using follow_invar'_parent_init
+  by unfold_locales
+
+subsubsection \<open>@{thm bfs_invar.invar_queue}\<close>
+
+lemma (in bfs) invar_queue_init:
+  shows "invar (queue init)"
+  using invar_empty
+  by (auto simp add: init_def intro: invar_snoc)
+
+subsubsection \<open>@{thm bfs_invar.queue_distinct}\<close>
+
+lemma (in bfs) queue_distinct_init:
+  shows "distinct (list (queue init))"
+  using invar_empty
+  by (simp add: init_def list_snoc list_empty)
+
+subsubsection \<open>@{thm bfs_invar.parent_src}\<close>
+
+lemma (in bfs) parent_src_init:
+  shows "parent init src = None"
+  by (simp add: init_def)
+
+subsubsection \<open>@{thm bfs_invar.gray_if_mem_queue}\<close>
+
+lemma (in bfs) gray_if_mem_queue_init:
+  assumes "v \<in> set (list (queue init))"
+  shows "gray init v"
+  using assms invar_empty
+  by (simp add: init_def list_snoc list_empty discovered_def)
+
+subsubsection \<open>@{thm bfs_invar.black_if_mem_ran}\<close>
+
+lemma (in bfs) black_if_mem_ran_init:
+  assumes "v \<in> ran (parent init)"
+  shows "black init v"
+  using assms
+  by (simp add: init_def)
+
+subsubsection \<open>@{thm bfs_invar.queue_sorted_wrt_dpath_length}\<close>
+
+lemma (in bfs) queue_sorted_wrt_dpath_length_init:
+  assumes "\<not> is_empty (queue init)"
+  shows
+    "sorted_wrt
+      (\<lambda>u v. dpath_length (rev (parent.follow (parent init) u)) \<le>
+             dpath_length (rev (parent.follow (parent init) v)))
+      (list (queue init)) \<and>
+     dpath_length (rev (parent.follow (parent init) (last (list (queue init))))) \<le>
+     dpath_length (rev (parent.follow (parent init) (head (queue init)))) + 1"
+  using invar_empty invar_queue_init
+  by (simp add: init_def list_snoc list_empty list_head)
+
+subsubsection \<open>@{thm bfs_invar.not_white_imp_shortest_dpath}\<close>
+
+lemma (in bfs) not_white_imp_shortest_dpath_init:
+  assumes "\<not> white init v"
+  shows
+    "dpath_bet G (rev (parent.follow (parent init) v)) src v \<and>
+     dpath_length (rev (parent.follow (parent init) v)) = dist v"
+proof -
+  have dpath_bet: "dpath_bet G [src] src src"
+    using src_in_vertices
+    by (intro dpath_bet_reflexive)
+  have "dpath_length [src] = 0"
+    by simp
+  also have "... \<le> dist src"
+    using zero_le
+    by (subst zero_enat_def[symmetric])
+  finally have "dpath_length [src] \<le> dist src"
+    .
+  hence "dpath_length [src] = dist src"
+    using dpath_bet
+    by (intro dist_le_dpath_length antisym)
+  moreover have "v = src"
+    using assms
+    by (simp add: discovered_def init_def)
+  moreover have "rev (parent.follow (parent init) src) = [src]"
+    using parent_init
+    by (simp add: parent_src_init parent.follow_psimps)
+  ultimately show ?thesis
+    using dpath_bet
+    by simp
+qed
+
+subsubsection \<open>@{thm bfs_invar.black_imp_out_neighborhood_not_white}\<close>
+
+lemma (in bfs) black_imp_out_neighborhood_not_white_init:
+  assumes "black init v"
+  shows "\<forall>w\<in>out_neighborhood G v. \<not> white init w"
+proof -
+  have "v = src"
+    using assms
+    by (simp add: discovered_def init_def)
+  moreover have "src \<in> set (list (queue init))"
+    using invar_empty
+    by (simp add: init_def list_snoc)
+  ultimately show ?thesis
+    using assms
+    by blast
+qed
+
+subsubsection \<open>\<close>
+
+lemma (in bfs) bfs_invar_init:
+  shows "bfs_invar empty is_empty head tail invar list src G snoc init"
+  using bfs_axioms
+  using follow_invar'_parent_init
+  using invar_queue_init queue_distinct_init parent_src_init gray_if_mem_queue_init
+  using black_if_mem_ran_init queue_sorted_wrt_dpath_length_init not_white_imp_shortest_dpath_init
+  using black_imp_out_neighborhood_not_white_init
+  by unfold_locales
+
+subsection \<open>@{term bfs.fold}\<close>
+
+subsubsection \<open>Convenience Lemmas\<close>
+
+lemma (in bfs_invar) list_queue_non_empty:
+  assumes "cond s"
+  shows "list (queue s) \<noteq> []"
+  using invar_queue assms
+  by (intro list_queue_non_empty)
+
+(* TODO: move somewhere else *)
+lemma (in Queue) list_queue:
+  assumes "invar q"
+  assumes "list q \<noteq> []"
+  shows "list q = head q # list (tail q)"
+  using assms
+  by (simp add: list_head list_tail)
+
+lemma (in bfs_invar) head_imp:
+  assumes cond: "cond s"
+  assumes v_eq_head: "v = head (queue s)"
+  shows
+    "v \<in> set (list (queue s))"
+    "v \<notin> set (list (queue (fold s)))"
+proof -
+  show "v \<in> set (list (queue s))"
+    using invar_queue assms list_queue_non_empty
+    by (simp add: list_head)
+  hence "v \<notin> set (filter (Not \<circ> discovered s) (sorted_list_of_set (out_neighborhood G (head (queue s)))))"
+    using gray_if_mem_queue
+    by fastforce
+  moreover have "v \<notin> set (list (tail (queue s)))"
+    using queue_distinct v_eq_head
+    by (simp add: list_queue[OF invar_queue list_queue_non_empty[OF cond]])
+  ultimately show "v \<notin> set (list (queue (fold s)))"
+    using invar_queue cond
+    by (simp add: list_queue_fold_cong_2)
+qed
+
+lemma (in bfs_invar) head_if:
+  assumes "cond s"
+  assumes "v \<in> set (list (queue s))"
+  assumes "v \<notin> set (list (queue (fold s)))"
+  shows "v = head (queue s)"
+proof -
+  have "list (queue s) = head (queue s) # list (tail (queue s))"
+    using invar_queue assms(1)
+    by (intro list_queue_non_empty list_queue)
+  thus ?thesis
+    using invar_queue assms
+    by (simp add: list_queue_fold_cong_2)
+qed
+
+lemma (in bfs_invar) head_iff:
+  assumes "cond s"
+  shows "v = head (queue s) \<longleftrightarrow> v \<in> set (list (queue s)) \<and> v \<notin> set (list (queue (fold s)))"
+proof (standard, goal_cases)
+  case 1
+  thus ?case
+    using assms
+    by (intro head_imp conjI)
+next
+  case 2
+  thus ?case
+    using assms
+    by (blast intro: head_if)
+qed
+
+lemma (in bfs_invar) not_white_imp_not_white_fold:
+  assumes "\<not> white s v"
+  shows "\<not> white (fold s) v"
+  using assms
+  by (auto simp add: discovered_def parent_fold_cong_2)
+
+subsubsection \<open>\<close>
+
+lemma (in bfs_invar) follow_invar'_parent_fold:
+  assumes "cond s"
+  shows "follow_invar' (parent (fold s))"
+  unfolding follow_invar'_def T_fold_cong_2
+proof (rule wf_Un[unfolded follow_invar'_def])
+  let ?r =
+    "{(head (queue s), v) |v.
+      v \<in> set (sorted_list_of_set (out_neighborhood G (head (queue s)))) \<and> \<not> discovered s v}"
+  show "wf (T s)"
+    using follow_invar'
+    by (simp add: follow_invar'_def)
+  have "gray s (head (queue s))"
+    using assms
+    by (intro head_imp(1) gray_if_mem_queue) simp+
+  thus "wf ?r"
+    by (simp add: wf_def)
+  show "Domain (T s) \<inter> Range ?r = {}"
+    using black_if_mem_ran
+    by (auto simp add: ran_def)
+qed
+
+lemma (in bfs_invar) parent_fold:
+  assumes "cond s"
+  shows "Tbd.parent (parent (fold s))"
+  using assms
+  by unfold_locales (intro follow_invar'_parent_fold)
+
+subsubsection \<open>@{thm bfs_invar.invar_queue}\<close>
+
+lemma (in bfs_invar) invar_queue_fold:
+  assumes "cond s"
+  shows "invar (queue (fold s))"
+  using invar_queue assms
+  by (intro invar_queue_fold_2)
+
+subsubsection \<open>@{thm bfs_invar.queue_distinct}\<close>
+
+lemma (in bfs_invar) queue_distinct_fold:
+  assumes "cond s"
+  shows "distinct (list (queue (fold s)))"
+proof -
+  let ?l1 = "(list (tail (queue s)))"
+  let ?l2 = "(filter (Not \<circ> discovered s) (sorted_list_of_set (out_neighborhood G (head (queue s)))))"
+  have list_queue_non_empty: "list (queue s) \<noteq> []"
+    using assms
+    by (intro list_queue_non_empty)
+  hence "\<And>v. v \<in> set ?l1 \<Longrightarrow> \<not> white s v"
+    using gray_if_mem_queue invar_queue
+    by (auto simp add: list_tail intro: list.set_sel(2))
+  hence "set ?l1 \<inter> set ?l2 = {}"
+    by fastforce
+  moreover have "distinct ?l1"
+    using queue_distinct invar_queue list_queue_non_empty
+    by (auto simp add: list_tail intro: distinct_tl)
+  moreover have "distinct ?l2"
+    by fastforce
+  ultimately show ?thesis
+    using invar_queue assms
+    by (simp add: list_queue_fold_cong_2)
+qed
+
+subsubsection \<open>@{thm bfs_invar.parent_src}\<close>
+
+lemma (in bfs_invar) parent_src_fold:
+  shows "parent (fold s) src = None"
+  using src_not_white
+  by (simp add: parent_fold_cong_2 parent_src)
+
+subsubsection \<open>@{thm bfs_invar.gray_if_mem_queue}\<close>
+
+lemma (in bfs_invar) gray_if_mem_queue_fold:
+  assumes cond: "cond s"
+  assumes mem_queue_fold: "v \<in> set (list (queue (fold s)))"
+  shows "gray (fold s) v"
+proof (cases "v \<in> set (list (queue s))")
+  case True
+  hence "gray s v"
+    by (intro gray_if_mem_queue)
+  thus ?thesis
+    using cond not_white_imp_not_white_fold mem_queue_fold
+    by blast
+next
+  case False
+  have "list (queue s) \<noteq> []"
+    using cond
+    by (intro list_queue_non_empty)
+  hence "v \<notin> set (list (tail (queue s)))"
+    using False invar_queue
+    by (auto simp add: list_tail intro: list.set_sel(2))
+  hence "v \<in> set (sorted_list_of_set (out_neighborhood G (head (queue s)))) \<and> \<not> discovered s v"
+    using mem_queue_fold invar_queue cond
+    by (simp add: list_queue_fold_cong_2)
+  hence "\<not> white (fold s) v"
+    by (fastforce simp add: discovered_def parent_fold_cong_2)
+  thus ?thesis
+    using mem_queue_fold
+    by blast
+qed
+
+subsubsection \<open>@{thm bfs_invar.black_if_mem_ran}\<close>
+
+lemma (in bfs_invar) black_if_mem_ran_fold_case_1:
+  assumes cond: "cond s"
+  assumes mem_ran: "v \<in> ran (parent s)"
+  shows "black (fold s) v"
+proof (rule ccontr)
+  assume assm: "\<not> black (fold s) v"
+  have black: "black s v"
+    using mem_ran
+    by (intro black_if_mem_ran)
+  with cond
+  have not_white_fold: "\<not> white (fold s) v"
+    by (intro black_imp_not_white not_white_imp_not_white_fold)
+  have "list (queue s) \<noteq> []"
+    using cond
+    by (intro list_queue_non_empty)
+  hence "v \<notin> set (list (tail (queue s)))"
+    using black invar_queue
+    by (auto simp add: list_tail intro: list.set_sel(2))
+  moreover have "v \<in> set (list (queue (fold s)))"
+    using assm not_white_fold
+    by blast
+  ultimately have "white (fold s) v"
+    using invar_queue cond black
+    by (simp add: discovered_def list_queue_fold_cong_2)
+  thus "False"
+    using not_white_fold
+    by blast
+qed
+
+lemma (in bfs_invar) black_if_mem_ran_fold_case_2_aux:
+  assumes "v \<notin> ran (parent s)"
+  assumes "v \<in> ran (parent (fold s))"
+  shows "v = head (queue s)"
+proof -
+  have
+    "dom (parent s) \<inter>
+     dom (\<lambda>v. if v \<in> set (sorted_list_of_set (out_neighborhood G (head (queue s)))) \<and> \<not> discovered s v
+              then Some (head (queue s)) else None) = {}"
+    by (auto simp add: domIff discovered_def)
+  hence
+    "ran (parent (fold s)) =
+     ran (parent s) \<union>
+     ran (\<lambda>v. if v \<in> set (sorted_list_of_set (out_neighborhood G (head (queue s)))) \<and> \<not> discovered s v
+              then Some (head (queue s)) else None)"
+    by (simp add: parent_fold_cong_2 ran_map_add)
+  thus ?thesis
+    using assms
+    by (auto simp add: ran_def split: if_splits(2))
+qed
+
+lemma (in bfs_invar) black_if_mem_ran_fold_case_2:
+  assumes cond: "cond s"
+  assumes mem_ran_fold: "v \<in> ran (parent (fold s))"
+  assumes not_mem_ran: "v \<notin> ran (parent s)"
+  shows "black (fold s) v"
+proof -
+  have v_eq_head_queue: "v = head (queue s)"
+    using invar_queue not_mem_ran mem_ran_fold
+    by (intro black_if_mem_ran_fold_case_2_aux)
+  hence "v \<in> set (list (queue s))"
+    using invar_queue cond
+    by (simp add: cond_def is_empty list_head)
+  hence "\<not> white s v"
+    by (intro gray_if_mem_queue gray_imp_not_white)
+  with cond
+  have "\<not> white (fold s) v"
+    by (intro not_white_imp_not_white_fold)
+  moreover have "v \<notin> set (list (queue (fold s)))"
+    using cond v_eq_head_queue
+    by (intro head_imp(2))
+  ultimately show ?thesis
+    by blast
+qed
+
+lemma (in bfs_invar) black_if_mem_ran_fold:
+  assumes "cond s"
+  assumes "v \<in> ran (parent (fold s))"
+  shows "black (fold s) v"
+proof (cases "v \<in> ran (parent s)")
+  case True
+  with assms(1)
+  show ?thesis
+    by (intro black_if_mem_ran_fold_case_1)
+next
+  case False
+  with assms
+  show ?thesis
+    by (intro black_if_mem_ran_fold_case_2)
+qed
+
+subsubsection \<open>@{thm bfs_invar.queue_sorted_wrt_dpath_length}\<close>
+subsubsection \<open>@{thm bfs_invar.not_white_imp_shortest_dpath}\<close>
+subsubsection \<open>@{thm bfs_invar.black_imp_out_neighborhood_not_white}\<close>
+
+subsubsection \<open>@{thm bfs_invar.queue_sorted_wrt_dpath_length}\<close>
+
+lemma (in bfs_invar) not_white_imp_follow_fold_eq_follow:
+  assumes "cond s"
+  assumes "\<not> white s v"
+  shows "parent.follow (parent (fold s)) v = follow v"
+  using assms
+proof (induct v rule: follow.pinduct[OF follow_dom])
+  case (1 v)
+  show ?case
+  proof (cases "v = src")
+    case True
+    hence
+      "parent s v = None"
+      "parent (fold s) v = None"
+      using parent_src "1.prems"(1) parent_src_fold
+      by simp+
+    hence
+      "follow v = [v]"
+      "parent.follow (parent (fold s)) v = [v]"
+      using "1.prems"(1) parent_fold
+      by (simp_all add: follow_psimps parent.follow_psimps)
+    thus ?thesis
+      by fastforce
+  next
+    case False
+    then obtain u where u:
+      "parent s v = Some u"
+      "\<not> white s u"
+      using False "1.prems"(2) black_if_mem_ran
+      by (auto simp add: discovered_def ran_def)
+    moreover hence "parent (fold s) v = Some u"
+      using "1.prems"
+      by (simp add: parent_fold_cong_2 map_add_Some_iff)
+    ultimately have
+      "follow v = v # follow u"
+      "parent.follow (parent (fold s)) v = v # parent.follow (parent (fold s)) u"
+      using "1.prems"(1) parent_fold
+      by (simp_all add: follow_psimps parent.follow_psimps)
+    thus ?thesis
+      using u "1.prems"(1)
+      by (simp add: "1.hyps"(2))
+  qed
+qed
+
+lemma (in bfs_invar) queue_sorted_wrt_dpath_length_fold_aux:
+  assumes "cond s"
+  shows
+    "\<forall>v\<in>set (filter (Not \<circ> discovered s) (sorted_list_of_set (out_neighborhood G (head (queue s))))).
+      parent.follow (parent (fold s)) v = v # parent.follow (parent (fold s)) (head (queue s))"
+proof
+  let ?u = "head (queue s)"
+  fix v
+  assume "v \<in> set (filter (Not \<circ> discovered s) (sorted_list_of_set (out_neighborhood G ?u)))"
+  hence "parent (fold s) v = Some ?u"
+    by (simp add: parent_fold_cong_2)
+  thus "parent.follow (parent (fold s)) v = v # parent.follow (parent (fold s)) ?u"
+    using assms parent_fold
+    by (simp add: parent.follow_psimps)
+qed
+
+lemma (in bfs_invar) queue_sorted_wrt_dpath_length_fold_aux_2:
+  assumes "cond s"
+  shows
+    "\<And>u v.
+      u \<in> set (filter (Not \<circ> discovered s) (sorted_list_of_set (out_neighborhood G (head (queue s))))) \<Longrightarrow>
+      v \<in> set (filter (Not \<circ> discovered s) (sorted_list_of_set (out_neighborhood G (head (queue s))))) \<Longrightarrow>
+      dpath_length (parent.follow (parent (fold s)) u) = dpath_length (parent.follow (parent (fold s)) v)"
+proof -
+  let ?u = "head (queue s)"
+  fix u v
+  assume
+    "u \<in> set (filter (Not \<circ> discovered s) (sorted_list_of_set (out_neighborhood G ?u)))"
+    "v \<in> set (filter (Not \<circ> discovered s) (sorted_list_of_set (out_neighborhood G ?u)))"
+  hence
+    "parent.follow (parent (fold s)) u = u # parent.follow (parent (fold s)) ?u" and
+    "parent.follow (parent (fold s)) v = v # parent.follow (parent (fold s)) ?u"
+    using assms queue_sorted_wrt_dpath_length_fold_aux
+    by blast+
+  hence
+    "dpath_length (parent.follow (parent (fold s)) u) = dpath_length (parent.follow (parent (fold s)) ?u) + 1"
+    "dpath_length (parent.follow (parent (fold s)) v) = dpath_length (parent.follow (parent (fold s)) ?u) + 1"
+    using assms parent_fold parent.follow_non_empty
+    by (fastforce simp add: dpath_length_Cons)+
+  thus "dpath_length (parent.follow (parent (fold s)) u) = dpath_length (parent.follow (parent (fold s)) v)"
+    by presburger
+qed
+
+lemma (in bfs_invar) queue_sorted_wrt_dpath_length_fold_aux_3:
+  assumes "cond s"
+  shows
+    "\<forall>v\<in>set (filter (Not \<circ> discovered s) (sorted_list_of_set (out_neighborhood G (head (queue s))))).
+      dpath_length (parent.follow (parent (fold s)) (last (list (queue s)))) \<le>
+      dpath_length (parent.follow (parent (fold s)) v)"
+proof
+  let ?u = "head (queue s)"
+  fix v
+  assume "v \<in> set (filter (Not \<circ> discovered s) (sorted_list_of_set (out_neighborhood G ?u)))"
+  hence follow_fold_eq: "parent.follow (parent (fold s)) v = v # parent.follow (parent (fold s)) ?u"
+    using assms queue_sorted_wrt_dpath_length_fold_aux
+    by blast
+  have
+    "dpath_length (parent.follow (parent (fold s)) (last (list (queue s)))) =
+      dpath_length (follow (last (list (queue s))))"
+    using assms list_queue_non_empty gray_if_mem_queue
+    by (simp add: not_white_imp_follow_fold_eq_follow)
+  also have "... \<le> dpath_length (follow ?u) + 1"
+    using assms queue_sorted_wrt_dpath_length
+    by (simp add: cond_def)
+  also have "... = dpath_length (parent.follow (parent (fold s)) ?u) + 1"
+    using assms head_imp(1) gray_if_mem_queue
+    by (simp add: not_white_imp_follow_fold_eq_follow)
+  also have "... = dpath_length (parent.follow (parent (fold s)) v)"
+    using assms parent_fold parent.follow_non_empty
+    by (fastforce simp add: follow_fold_eq dpath_length_Cons)
+  finally show
+    "dpath_length (parent.follow (parent (fold s)) (last (list (queue s)))) \<le>
+      dpath_length (parent.follow (parent (fold s)) v)"
+    .
+qed
+
+lemma (in bfs_invar) queue_sorted_wrt_dpath_length_fold_aux_4:
+  assumes "cond s"
+  shows
+    "\<forall>u\<in>set (list (tail (queue s))).
+      \<forall>v\<in>set (filter (Not \<circ> discovered s) (sorted_list_of_set (out_neighborhood G (head (queue s))))).
+      dpath_length (parent.follow (parent (fold s)) u) \<le> dpath_length (parent.follow (parent (fold s)) v)"
+proof (standard, standard)
+  let ?u = "head (queue s)"
+  let ?q = "tail (queue s)"
+  fix u v
+  assume "u \<in> set (list ?q)"
+  hence u_mem_list_queue: "u \<in> set (list (queue s))"
+    using invar_queue assms list_queue_non_empty
+    by (auto simp add: list_tail intro: list.set_sel(2))
+  assume v_mem_filter: "v \<in> set (filter (Not \<circ> discovered s) (sorted_list_of_set (out_neighborhood G ?u)))"
+  have
+    "dpath_length (parent.follow (parent (fold s)) u) =
+      dpath_length (follow u)"
+    using assms u_mem_list_queue gray_if_mem_queue
+    by (simp add: not_white_imp_follow_fold_eq_follow)
+  also have "... \<le> dpath_length (follow (last (list (queue s))))"
+    using u_mem_list_queue
+    by (intro mem_queue_imp_dpath_length_last_queue)
+  also have "... = dpath_length (parent.follow (parent (fold s)) (last (list (queue s))))"
+    using assms list_queue_non_empty gray_if_mem_queue
+    by (simp add: not_white_imp_follow_fold_eq_follow)
+  also have "... \<le> dpath_length (parent.follow (parent (fold s)) v)"
+    using assms v_mem_filter queue_sorted_wrt_dpath_length_fold_aux_3
+    by blast
+  finally show
+    "dpath_length (parent.follow (parent (fold s)) u) \<le>
+      dpath_length (parent.follow (parent (fold s)) v)"
+    .
+qed
+
+lemma (in bfs_invar) aux_0:
+  assumes cond: "cond s"
+  assumes "\<not> is_empty (queue (fold s))"
+  shows
+    "dpath_length (parent.follow (parent (fold s)) (last (list (queue (fold s))))) \<le>
+      dpath_length (parent.follow (parent (fold s)) (head (queue s))) + 1"
+proof (cases "filter (Not \<circ> discovered s) (sorted_list_of_set (out_neighborhood G (head (queue s)))) = []")
+  case True
+  hence list_tail_non_empty: "list (tail (queue s)) \<noteq> []"
+    using invar_queue assms invar_queue_fold_2
+    by (simp add: list_queue_fold_cong_2 is_empty)
+  hence "last (list (queue (fold s))) = last (list (tail (queue s)))"
+    unfolding list_queue_fold_cong_2[OF invar_queue assms(1)] last_appendL[OF True]
+    by blast
+  hence "last (list (queue (fold s))) = last (list (queue s))"
+    using list_tail_non_empty
+    by (simp add: list_queue[OF invar_queue list_queue_non_empty[OF assms(1)]])
+  hence
+    "dpath_length (parent.follow (parent (fold s)) (last (list (queue (fold s))))) =
+      dpath_length (follow (last (list (queue s))))"
+    using cond list_queue_non_empty gray_if_mem_queue
+    by (simp add: not_white_imp_follow_fold_eq_follow)
+  also have "... \<le> dpath_length (follow (head (queue s))) + 1"
+    using invar_queue cond list_queue_non_empty queue_sorted_wrt_dpath_length
+    by (simp add: is_empty)
+  also have "... = dpath_length (parent.follow (parent (fold s)) (head (queue s))) + 1"
+    using cond head_imp(1) gray_if_mem_queue
+    by (simp add: not_white_imp_follow_fold_eq_follow)
+  finally show ?thesis
+    .
+next
+  case False
+  hence
+    "last (list (queue (fold s))) \<in>
+      set (filter (Not \<circ> discovered s) (sorted_list_of_set (out_neighborhood G (head (queue s)))))"
+    unfolding list_queue_fold_cong_2[OF invar_queue cond] last_appendR[OF False]
+    by (intro last_in_set)
+  hence
+    "parent.follow (parent (fold s)) (last (list (queue (fold s)))) =
+      (last (list (queue (fold s)))) # parent.follow (parent (fold s)) (head (queue s))"
+    using cond queue_sorted_wrt_dpath_length_fold_aux
+    by blast
+  thus ?thesis
+    using cond parent_fold parent.follow_non_empty
+    by (fastforce simp add: dpath_length_Cons)
+qed
+
+lemma (in bfs_invar) aux_1:
+  assumes "cond s"
+  assumes "\<not> is_empty (queue (fold s))"
+  assumes "list (tail (queue s)) = []"
+  shows
+    "head (queue (fold s)) \<in>
+      set (filter (Not \<circ> discovered s) (sorted_list_of_set (out_neighborhood G (head (queue s)))))"
+proof -
+  have "head (queue (fold s)) = hd (list (queue (fold s)))"
+    using assms(1, 2) invar_queue invar_queue_fold_2
+    by (simp add: is_empty list_head)
+  hence
+    "head (queue (fold s)) =
+    hd (filter (Not \<circ> discovered s) (sorted_list_of_set (out_neighborhood G (head (queue s)))))"
+    using invar_queue assms(1, 3)
+    by (simp add: list_queue_fold_cong_2)
+  moreover have "filter (Not \<circ> discovered s) (sorted_list_of_set (out_neighborhood G (head (queue s)))) \<noteq> []"
+    using invar_queue assms invar_queue_fold_2
+    by (simp add: is_empty list_queue_fold_cong_2)
+  ultimately show ?thesis
+    using list.set_sel(1)
+    by metis
+qed
+
+lemma (in bfs_invar) aux_2:
+  assumes cond: "cond s"
+  assumes "\<not> is_empty (queue (fold s))"
+  shows
+    "dpath_length (parent.follow (parent (fold s)) (head (queue s))) \<le>
+      dpath_length (parent.follow (parent (fold s)) (head (queue (fold s))))"
+proof (cases "list (tail (queue s)) = []")
+  case True
+  have
+    "dpath_length (parent.follow (parent (fold s)) (head (queue s))) =
+      dpath_length (follow (head (queue s)))"
+    using cond head_imp(1) gray_if_mem_queue
+    by (simp add: not_white_imp_follow_fold_eq_follow)
+  also have "... \<le> dpath_length (follow (last (list (queue s))))"
+    using cond
+    by (intro head_imp(1) mem_queue_imp_dpath_length_last_queue) simp+
+  also have "... = dpath_length (parent.follow (state.parent (local.fold s)) (last (list (queue s))))"
+    using cond list_queue_non_empty gray_if_mem_queue
+    by (simp add: not_white_imp_follow_fold_eq_follow)
+  also have "... \<le> dpath_length (parent.follow (parent (fold s)) (head (queue (fold s))))"
+    using assms True aux_1 queue_sorted_wrt_dpath_length_fold_aux_3
+    by blast
+  finally show ?thesis
+    .
+next
+  case False
+  have "head (queue (fold s)) = hd (list (queue (fold s)))"
+    using assms invar_queue invar_queue_fold_2
+    by (simp add: is_empty list_head)
+  hence "head (queue (fold s)) = hd (list (tail (queue s)))"
+    using invar_queue cond False
+    by (simp add: list_queue_fold_cong_2)
+  hence head_queue_fold_mem_list_queue: "head (queue (fold s)) \<in> set (list (queue s))"
+    using False invar_queue cond list_queue_non_empty
+    by (auto simp add: list_tail intro: list.set_sel(2))
+
+  have
+    "dpath_length (parent.follow (parent (fold s)) (head (queue s))) =
+      dpath_length (follow (head (queue s)))"
+    using cond head_imp(1) gray_if_mem_queue
+    by (simp add: not_white_imp_follow_fold_eq_follow)
+  also have "... \<le> dpath_length (follow (head (queue (fold s))))"
+    using head_queue_fold_mem_list_queue
+    by (intro mem_queue_imp_dpath_length_head_queue)
+  also have "... = dpath_length (parent.follow (parent (fold s)) (head (queue (fold s))))"
+    using cond head_queue_fold_mem_list_queue gray_if_mem_queue
+    by (simp add: not_white_imp_follow_fold_eq_follow)
+  finally show ?thesis
+    .
+qed
+
+(* TODO: move somewhere else *)
+lemma sorted_wrt_if:
+  assumes "\<And>x y. x \<in> set l \<Longrightarrow> y \<in> set l \<Longrightarrow> P x y"
+  shows "sorted_wrt P l"
+  using assms
+  by (simp add: sorted_wrt_iff_nth_less)
+
+lemma (in bfs_invar) queue_sorted_wrt_dpath_length_fold_aux_5:
+  assumes "cond s"
+  shows
+    "sorted_wrt
+      (\<lambda>u v. dpath_length (parent.follow (parent (fold s)) u) \<le>
+             dpath_length (parent.follow (parent (fold s)) v))
+      (list (tail (queue s)))"
+proof -
+  have list_queue_non_empty: "list (queue s) \<noteq> []"
+    using assms
+    by (intro list_queue_non_empty)
+  hence "sorted_wrt (\<lambda>u v. dpath_length (follow u) \<le> dpath_length (follow v)) (list (queue s))"
+    using invar_queue queue_sorted_wrt_dpath_length
+    by (simp add: is_empty)
+  hence
+    "sorted_wrt
+      (\<lambda>u v. dpath_length (parent.follow (parent (fold s)) u) \<le>
+             dpath_length (parent.follow (parent (fold s)) v))
+      (list (queue s))"
+    using assms gray_if_mem_queue sorted_wrt_mono_rel[of "(list (queue s))"]
+    by (simp add: not_white_imp_follow_fold_eq_follow)
+  thus ?thesis
+    by (simp add: list_queue[OF invar_queue list_queue_non_empty])
+qed
+
+lemma (in bfs_invar) queue_sorted_wrt_dpath_length_fold:
+  assumes "cond s"
+  assumes "\<not> is_empty (queue (fold s))"
+  shows
+    "sorted_wrt
+      (\<lambda>u v. dpath_length (parent.follow (parent (fold s)) u) \<le>
+             dpath_length (parent.follow (parent (fold s)) v))
+      (list (queue (fold s))) \<and>
+     dpath_length (parent.follow (parent (fold s)) (last (list (queue (fold s))))) \<le>
+     dpath_length (parent.follow (parent (fold s)) (head (queue (fold s)))) + 1"
+proof (rule conjI)
+  have
+    "\<And>u v.
+      u \<in> set (filter (Not \<circ> discovered s) (sorted_list_of_set (out_neighborhood G (head (queue s))))) \<Longrightarrow>
+      v \<in> set (filter (Not \<circ> discovered s) (sorted_list_of_set (out_neighborhood G (head (queue s))))) \<Longrightarrow>
+      dpath_length (parent.follow (parent (fold s)) u) \<le> dpath_length (parent.follow (parent (fold s)) v)"
+    using assms(1)
+    by (blast intro: queue_sorted_wrt_dpath_length_fold_aux_2 eq_imp_le)
+  hence
+    "sorted_wrt
+      (\<lambda>u v. dpath_length (parent.follow (parent (fold s)) u) \<le>
+             dpath_length (parent.follow (parent (fold s)) v))
+      (filter (Not \<circ> discovered s) (sorted_list_of_set (out_neighborhood G (head (queue s)))))"
+    by (blast intro: sorted_wrt_if)
+  thus
+    "sorted_wrt
+      (\<lambda>u v. dpath_length (parent.follow (parent (fold s)) u) \<le>
+             dpath_length (parent.follow (parent (fold s)) v))
+      (list (queue (fold s)))"
+    using invar_queue assms(1) queue_sorted_wrt_dpath_length_fold_aux_5 queue_sorted_wrt_dpath_length_fold_aux_4
+    by (simp add: list_queue_fold_cong_2 sorted_wrt_append)
+
+  have
+    "dpath_length (parent.follow (parent (fold s)) (last (list (queue (fold s))))) \<le>
+      dpath_length (parent.follow (parent (fold s)) (head (queue s))) + 1"
+    using assms
+    by (intro aux_0)
+  also have "... \<le> dpath_length (parent.follow (parent (fold s)) (head (queue (fold s)))) + 1"
+    using assms
+    by (auto intro: aux_2)
+  finally show
+    "dpath_length (parent.follow (parent (fold s)) (last (list (queue (fold s))))) \<le>
+      dpath_length (parent.follow (parent (fold s)) (head (queue (fold s)))) + 1"
+    .
+qed
+
+subsubsection \<open>@{thm bfs_invar.not_white_imp_shortest_dpath}\<close>
+
+lemma (in bfs_invar) parent_fold_eq_head_queue_if:
+  assumes "white s v"
+  assumes "\<not> white (fold s) v"
+  shows "parent (fold s) v = Some (head (queue s))"
+proof -
+  have
+    "parent (fold s) v =
+      (\<lambda>v. if v \<in> set (sorted_list_of_set (out_neighborhood G (head (queue s)))) \<and> white s v then Some (head (queue s)) else None) v"
+    using assms(1)
+    by (simp add: discovered_def domIff parent_fold_cong_2)
+  thus ?thesis
+    using assms
+    by (auto simp add: discovered_def)
+qed
+
+lemma (in bfs_invar) not_white_imp_shortest_dpath_2:
+  shows "\<And>v. \<not> white s v \<Longrightarrow> dpath_bet G (rev (follow v)) src v \<and> dpath_length (rev (follow v)) = dist v"
+  sorry
+
+thm bfs_invar.not_white_imp_shortest_dpath
+lemma (in bfs_invar) not_white_imp_shortest_dpath_fold:
+  assumes cond: "cond s"
+  assumes not_white_fold: "\<not> white (fold s) v"
+  assumes not_white_imp_shortest_dpath:
+    "\<And>v. \<not> white s v \<Longrightarrow> dpath_bet G (rev (follow v)) src v \<and> dpath_length (rev (follow v)) = dist v"
+  shows
+    "dpath_bet G (rev (parent.follow (parent (fold s)) v)) src v \<and>
+      dpath_length (rev (parent.follow (parent (fold s)) v)) = dist v"
+proof (cases "white s v")
+  case True
+  let ?u = "head (queue s)"
+  have *: "parent (fold s) v = Some ?u"
+    using True not_white_fold
+    by (intro parent_fold_eq_head_queue_if)
+
+  have **: "\<not> white s ?u"
+    using cond
+    by (intro head_imp(1) gray_if_mem_queue gray_imp_not_white) simp+
+  hence ****: "dpath_bet G (rev (follow ?u)) src ?u \<and> dpath_length (rev (follow ?u)) = dist ?u"
+    by (intro not_white_imp_shortest_dpath)
+
+  have "parent.follow (parent (fold s)) v = v # parent.follow (parent (fold s)) ?u"
+    using cond parent_fold
+    by (simp add: parent.follow_psimps *)
+  hence "parent.follow (parent (fold s)) v = v # follow ?u"
+    using cond **
+    by (simp add: not_white_imp_follow_fold_eq_follow)
+  hence ***: "rev (parent.follow (parent (fold s)) v) = rev (follow ?u) @ [v]"
+    by simp
+
+  have *****: "dpath_bet G [?u, v] ?u v"
+    sorry
+  hence 6: "dpath_bet G (rev (parent.follow (parent (fold s)) v)) src v"
+    using **** dpath_bet_transitive
+    by (fastforce simp add: ***)
+  have "dpath_length (rev (parent.follow (parent (fold s)) v)) = dpath_length (rev (follow ?u)) + 1"
+    using follow_non_empty
+    by (simp add: *** dpath_length_snoc)
+  also have "... = dist ?u + 1"
+    unfolding plus_enat_simps(1)[symmetric]
+    by (simp add: ****)
+  finally have 10: "dpath_length (rev (parent.follow (parent (fold s)) v)) = dist ?u + 1"
+    .
+  have 11: "dist ?u + 1 \<ge> dist v"
+    using ***** rename_me
+    by (simp add: edge_iff_dpath_bet)
+  
+  have "reachable G src v"
+    using 6
+    by (auto simp add: reachable_iff_dpath_bet)
+  then obtain p where p:
+    "dpath_bet G p src v"
+    "dpath_length p = dist v"
+    by (elim dist_dpath_betE)
+  have "dist ?u + 1 = dist v"
+  proof (rule ccontr)
+    assume "dist ?u + 1 \<noteq> dist v"
+    hence 7: "dist v < dist ?u + 1"
+      using 11
+      by auto
+    thus "False"
+      using True p
+    proof (induct p arbitrary: v rule: dpath_rev_induct)
+      case 1
+      thus ?case
+        by auto
+    next
+      case (2 u)
+      hence "[u] = [src] \<and> src = v"
+        by (intro hd_of_dpath_bet' last_of_dpath_bet list_length_1) simp
+      hence "white s src"
+        using "2.prems"(2)
+        by simp
+      thus ?case
+        by (simp add: discovered_def)
+    next
+      case (3 u u' l)
+      have "dist u + 1 = dist v"
+        using "3.prems"(3, 4)
+        by (auto intro: shortest_dpathE_2)
+      also have "... < dist ?u + 1"
+        using "3.prems"(1)
+        .
+      finally have "dist u + 1 < dist ?u + 1"
+        .
+      hence 9: "dist u < dist ?u"
+        unfolding plus_1_eSuc(2) eSuc_mono
+        .
+      show ?case
+      proof (induct s u rule: vertex_color_induct)
+        case white
+        have "dist ?u \<le> dist (last (list (queue s)))"
+          using cond list_queue_non_empty
+          by (intro mem_queue_imp_dist_head_queue) simp
+        also have "... \<le> dist u"
+          using white cond white_imp_dist_ge
+          by (simp add: cond_def)
+        finally show ?case
+          using 9
+          by simp
+      next
+        case gray
+        hence "dist ?u \<le> dist u"
+          by (intro mem_queue_imp_dist_head_queue) simp
+        thus ?case
+          using 9
+          by simp
+      next
+        case black
+        have "dpath_bet G [u, v] u v"
+          using "3.prems"(3) split_dpath last_of_dpath_bet
+          by fastforce
+        hence "v \<in> out_neighborhood G u"
+          by (simp add: edge_iff_dpath_bet in_out_neighborhood_iff_edge)
+        hence "\<not> white s v"
+          using black black_imp_out_neighborhood_not_white
+          by blast
+        thus ?case
+          using "3.prems"(2)
+          by simp
+      qed
+    qed
+  qed
+  thus ?thesis
+    using 6
+    by (simp add: 10)
+next
+  case False
+  thus ?thesis
+    using assms not_white_imp_shortest_dpath
+    by (simp add: not_white_imp_follow_fold_eq_follow)
+qed
+
+subsubsection \<open>@{thm bfs_invar.black_imp_out_neighborhood_not_white}\<close>
+
+(* TODO: remove? *)
+lemma (in bfs)
+  shows "\<forall>v\<in>out_neighborhood G (head (queue s)). \<not> white (fold s) v"
+  using out_neighborhood_finite
+  by (auto simp add: discovered_def parent_fold_cong_2)
+
+lemma (in bfs_invar) black_imp_out_neighborhood_not_white_fold:
+  assumes cond: "cond s"
+  assumes black_fold: "black (fold s) v"
+  shows "\<forall>w\<in>out_neighborhood G v. \<not> white (fold s) w"
+proof (induct s v rule: vertex_color_induct)
+  case white
+  hence "v \<in> set (sorted_list_of_set (out_neighborhood G (head (queue s))))"
+    using black_fold
+    by (fastforce simp add: discovered_def parent_fold_cong_2)
+  hence "v \<in> set (list (queue (fold s)))"
+    using white invar_queue cond
+    by (simp add: discovered_def list_queue_fold_cong_2)
+  thus ?case
+    using black_fold
+    by blast
+next
+  case gray
+  hence "v = head (queue s)"
+    using assms invar_queue
+    by (intro head_if) simp+
+  thus ?case
+    using out_neighborhood_finite
+    by (auto simp add: discovered_def parent_fold_cong_2)
+next
+  case black
+  hence "\<forall>w\<in>out_neighborhood G v. \<not> white s w"
+    by (intro black_imp_out_neighborhood_not_white)
+  thus ?case
+    using cond not_white_imp_not_white_fold
+    by blast
+qed
+
+lemma (in bfs_invar) bfs_invar_fold:
+  shows "bfs_invar empty is_empty head tail invar list src G snoc (fold s)"
+  sorry
+
+subsection \<open>@{term bfs.loop}\<close>
+
+subsubsection \<open>@{thm bfs_invar.invar_queue}\<close>
+subsubsection \<open>@{thm bfs_invar.dom_parent_subset_vertices}\<close>
+subsubsection \<open>@{thm bfs_invar.black_if_mem_ran}\<close>
+subsubsection \<open>@{thm bfs_invar.gray_if_mem_queue}\<close>
+subsubsection \<open>@{thm bfs_invar.queue_distinct}\<close>
+subsubsection \<open>@{thm bfs_invar.queue_sorted_wrt_dpath_length}\<close>
+subsubsection \<open>@{thm bfs_invar.not_white_imp_shortest_dpath}\<close>
+subsubsection \<open>@{thm bfs_invar.black_imp_out_neighborhood_not_white}\<close>
+subsubsection \<open>@{thm bfs_invar.parent_src}\<close>
+
+lemma (in bfs_invar) bfs_invar_fold:
+  shows "bfs_invar empty is_empty head tail invar list src G snoc (fold s)"
+  sorry
+
+lemma (in bfs_invar) bfs_invar_loop:
+  shows "bfs_invar empty is_empty head tail invar list src G snoc (loop s)"
+  sorry
+
+(**)
+
+lemma (in bfs) bfs_invar_init_2:
+  shows "bfs_invar empty is_empty head tail invar list src G snoc init"
+  sorry
+
+lemma (in bfs) bfs_invar_bfs:
+  shows "bfs_invar empty is_empty head tail invar list src G snoc bfs"
+  using bfs_invar_init bfs_invar.bfs_invar_loop
+  by fast
+
+section \<open>Correctness\<close>
+
+(**)
+
+lemma (in bfs) loop_psimps:
+  assumes "invar (queue s)"
+  assumes "dom (parent s) \<subseteq> dVs G"
+  shows "loop s = (if cond s then loop (fold s) else s)"
+  using loop.psimps[OF loop_dom[OF assms]]
+  by meson
+
+lemma (in bfs) bfs_induct:
+  assumes "invar (queue s)"
+  assumes "dom (parent s) \<subseteq> dVs G"
+  assumes
+    "\<And>s. loop_dom s \<Longrightarrow>
+          (cond s \<Longrightarrow>
+            P (fold s)) \<Longrightarrow>
+          P s"
+  shows "P s"
+  using assms
+  by (blast intro: loop_dom loop.pinduct)
+
+lemma (in bfs) bfs_induct_2:
+  assumes "bfs_invar empty is_empty head tail invar list src G snoc s"
+  assumes
+    "\<And>s. loop_dom s \<Longrightarrow>
+          (cond s \<Longrightarrow>
+            P (fold s)) \<Longrightarrow>
+          P s"
+  shows "P s"
+  using assms
+proof -
+  have "invar (queue s)"
+    using assms(1)
+    by (intro bfs_invar.invar_queue)
+  moreover have "dom (parent s) \<subseteq> dVs G"
+    using assms(1)
+    by (intro bfs_invar.dom_parent_subset_vertices)
+  ultimately show ?thesis
+    using assms(2)
+    by (rule bfs_induct)
+qed
+
+lemma (in bfs) sound:
+  assumes "bfs_invar empty is_empty head tail invar list src G snoc s"
+  assumes "discovered (loop s) v"
+  shows
+    "dpath_bet G (rev (parent.follow (parent (loop s)) v)) src v \<and>
+      dpath_length (rev (parent.follow (parent (loop s)) v)) = dist v"
+  using assms bfs_invar.bfs_invar_loop bfs_invar.not_white_imp_shortest_dpath_2
+  by fast
+
+lemma (in bfs_invar) sound:
+  assumes "discovered (loop s) v"
+  shows
+    "dpath_bet G (rev (parent.follow (parent (loop s)) v)) src v \<and>
+      dpath_length (rev (parent.follow (parent (loop s)) v)) = dist v"
+  using assms bfs_invar_loop bfs_invar.not_white_imp_shortest_dpath_2
+  by fast
+
+lemma (in bfs_invar) white_loop_imp_white:
+  assumes "white (loop s) v"
+  shows "white s v"
+  using assms
+  sledgehammer
+  by (metis discovered_def hd_of_dpath_bet not_white_imp_shortest_dpath parent.follow_ConsD parent_axioms)
+
+lemma (in bfs) bfs_complete:
+  assumes "bfs_invar empty is_empty head tail invar list src G snoc s"
+  assumes "\<not> discovered (loop s) v"
+  shows "\<not> reachable G src v"
+  using assms
+proof (induct rule: bfs_induct_2[OF assms(1)])
+  thm bfs_invar.not_white_imp_not_white_fold
+  case (1 s)
+  show ?case
+  proof (cases "cond s")
+    case True
+    hence *: "loop s = loop (fold s)"
+      using "1.hyps"(1)
+      by (metis loop.psimps surjective update_convs(1))
+    have "bfs_invar empty is_empty head tail invar list src G snoc (loop (fold s))"
+      using "1.prems"(1)
+      sledgehammer
+      using "*" bfs_invar.bfs_invar_loop by force
+    moreover have "white (loop (fold s)) v"
+      using "1.prems"
+      by (simp add: *)
+    ultimately show ?thesis
+      using True
+      sledgehammer
+      by (simp add: True \<open>bfs_invar empty is_empty head tail invar list src G snoc (loop (local.fold s))\<close> \<open>white (loop (local.fold s)) v\<close> "1.hyps"(2) "1.prems"(1) bfs_invar.bfs_invar_fold)
+  next
+    case False
+    thus ?thesis
+      by (metis "1.hyps"(1) "1.prems"(1) "1.prems"(2) bfs.loop.psimps bfs_axioms bfs_invar.invar_queue bfs_invar.src_not_white bfs_invar.tbd cond_def empty_iff is_empty list.set(1) reachable_iff_dpath_bet)
+  qed
+qed
+
+lemma (in bfs_invar) sound:
+  assumes "v \<noteq> src"
+  assumes "bfs_invar empty is_empty head tail invar list src G snoc s"
+  assumes "(parent.follow (parent (loop s)) v) \<noteq> [v]"
+  shows "dpath_bet G (parent.follow (parent (loop s)) v) src v"
+    "dpath_length (parent.follow (parent (loop s)) v) = dist v"
+
+lemma (in bfs_invar) sound:
+  assumes "v \<noteq> src"
+  assumes "bfs_invar empty is_empty head tail invar list src G snoc s"
+  assumes "dpath_bet G p src v"
+  shows "dpath_length p \<ge> dist v"
+  thm white_imp_dist_ge
+
+lemma (in bfs) bfs_sound:
+  assumes "discovered bsf v"
+  shows "dpath_bet G (parent.follow (parent bfs) v) src v \<and> dpath_length (parent.follow (parent bfs) v) = dist v"
+proof -
+  have "\<not> white bfs v"
+    using assms
+    by (simp add: domIff discovered_def)
+  with bfs_invar_bfs
+  show ?thesis
+    by (intro bfs_invar.not_white_imp_shortest_dpath)
+qed
+
+lemma (in bfs) bfs_complete:
+  assumes "\<not> discovered bfs v"
+  shows "\<not> reachable G src v"
+  sorry
+
+lemma (in bfs) bfs_correct:
+  shows
+    "if discovered bfs v
+     then dpath_bet G (parent.follow (parent bfs) v) src v \<and>
+          dpath_length (parent.follow (parent bfs) v) = dist v
+     else \<not> reachable G src v"
+  using bfs_complete bfs_sound
+  by (simp split: option.split)
+
+(**)
+
+subsection \<open>init\<close>
+
+
+subsection \<open>bfs\<close>
+
+lemma (in bfs) discovered_imp_shortest_dpath_fold:
+  assumes "cond s"
+  assumes "invar (queue s)"
+  assumes "dom (parent s) \<subseteq> dVs G"
+  assumes
+    "discovered s v \<Longrightarrow>
+      dpath_bet G (parent.follow (parent s) v) src v \<and>
+      dpath_length (parent.follow (parent s) v) = dist G src v"
+  shows
+    "discovered v (fold s) \<Longrightarrow>
+      dpath_bet G (parent.follow (parent (fold s)) v) src v \<and>
+      dpath_length (parent.follow (parent (fold s)) v) = dist G src v"
+  sorry
+
+lemma (in bfs) discovered_imp_shortest_dpath_loop:
+  assumes "invar (queue s)"
+  assumes "dom (parent s) \<subseteq> dVs G"
+  assumes
+    "discovered s v \<Longrightarrow>
+      dpath_bet G (parent.follow (parent s) v) src v \<and>
+      dpath_length (parent.follow (parent s) v) = dist G src v"
+  shows
+    "discovered v (loop s) \<Longrightarrow>
+      dpath_bet G (parent.follow (parent (loop s)) v) src v \<and>
+      dpath_length (parent.follow (parent (loop s)) v) = dist G src v"
+  using assms
+  proof (induct rule: bfs_induct[OF assms(1, 2)])
+  case (1 s)
+  thus ?case
+  proof (cases "cond s")
+    case True
+    hence loop:
+      "loop s =
+        loop (Finite_Set.fold (traverse_edge (head (queue s))) (s\<lparr>queue := tail (queue s)\<rparr>) (out_neighborhood G (head (queue s))))"
+      unfolding loop.psimps[OF "1.hyps"(1)]
+      by metis
+    thus ?thesis
+      using True "1.prems"
+      unfolding loop
+      by (intro tbd discovered_imp_shortest_dpath_fold "1.hyps"(2))
+  next
+    case False
+    thus ?thesis
+      using "1.prems"(1, 4) "1.hyps"(1)
+      by (simp add: loop.psimps)
+  qed
+qed
+
+lemma (in bfs_invar) discovered_imp_shortest_dpath_loop:
+  assumes "discovered v (loop s)"
+  shows
+    "dpath_bet G (parent.follow (parent (loop s)) v) src v \<and>
+      dpath_length (parent.follow (parent (loop s)) v) = dist G src v"
+  using invar_queue dom_parent_subset_vertices discovered_imp_shortest_dpath assms
+  by (intro discovered_imp_shortest_dpath_loop)
+
+lemma (in bfs) discovered_imp_shortest_dpath_bfs:
+  assumes "discovered v bfs"
+  shows
+    "dpath_bet G (parent.follow (parent bfs) v) src v \<and>
+      dpath_length (parent.follow (parent bfs) v) = dist G src v"
+  using bfs_invar_init assms
+  by (intro bfs_invar.discovered_imp_shortest_dpath_loop)
+
+(**)
+
+lemma (in bfs_invar)
+  assumes "\<not> discovered s v"
+  shows "(if is_empty (queue s) then \<infinity> else dist (last (list (queue s)))) \<le> dist v"
+proof (cases "reachable G src v")
+  case True
+  then obtain p where
+    "dpath_bet G p src v"
+    "dpath_length p = dist v"
+    sorry
+  thus ?thesis
+    using assms
+  proof (induct p arbitrary: v rule: dpath_rev_induct)
+    case 1
+    then show ?case sorry
+  next
+    case (2 w)
+    then show ?case sorry
+  next
+    case (3 w w' l)
+    consider
+    (white) "\<not> discovered w s" |
+    (gray) "discovered w s \<and> w \<in># mset (list (queue s))" |
+    (black) "discovered w s \<and> w \<notin># mset (list (queue s))"
+    by blast
+    thus ?case
+    proof (cases)
+      case white
+      then show ?thesis sorry
+    next
+      case gray
+      then show ?thesis sorry
+next
+  case black
+  then show ?thesis sorry
+qed
+  qed
+next
+  case False
+  then show ?thesis sorry
+qed
+
+lemma (in bfs_invar)
+  assumes "\<not> discovered s v"
+  assumes "distinct_dpath_bet G p src v"
+  shows "\<exists>v\<in>set p. v \<in># mset (list (queue s))"
+  using assms
+proof (induct p arbitrary: src rule: dpath_induct)
+  case 1
+  thus ?case
+    by (simp add: distinct_dpath_bet_def)
+next
+  case (2 u)
+  hence "dpath_bet G [u] src v"
+    by (simp add: distinct_dpath_bet_def)
+  hence "[u] = [src] \<and> src = v"
+    using "2.prems"(2)
+    by (intro hd_of_dpath_bet' last_of_dpath_bet list_length_1) simp
+  hence "\<not> discovered src s"
+    using "2.prems"(1)
+    by simp
+  thus ?case
+    using parent_src discovered_def
+    sledgehammer
+    by (simp add: discovered_def)
+next
+  case (3 u u' l)
+  hence "v \<noteq> u'"
+    thm dpath.induct
+    thm last_of_dpath_bet
+    apply (simp add: distinct_dpath_bet_def)
+  then show ?case sorry
+qed
+
+
+lemma (in bfs)
+  assumes "\<not> discovered v (fold s)"
+  assumes "dpath_bet G p (head (queue s)) v"
+  shows "\<exists>v\<in>set p. v \<in># mset (list (queue (fold s)))"
+  using assms
+proof (induct p arbitrary: v rule: dpath_induct)
+  case 1
+  thus ?case
+    by simp
+next
+  case (2 v)
+  thus ?case
+    sledgehammer
+next
+  case (3 v v' l)
+  then show ?case sorry
+qed
+
+lemma (in bfs) bsf_complete:
+  assumes "reachable G src v"
+  shows "discovered v bsf"
+  sorry
+
+locale bfs_invar = bfs where G = G and snoc = snoc
+  for
+    G :: "'a dgraph" and
+    snoc :: "'q \<Rightarrow> 'a \<Rightarrow> 'q" +
+  fixes s :: "('q, 'a) state"
   assumes distance_src: "distance s src = Some 0"
-  assumes parent_src: "parent s src = Some src"
+  assumes parent_src: "parent s src = None"
+  assumes invar_queue: "invar (queue s)"
+  assumes queue_subset_vertices: "set (list (queue s)) \<subseteq> dVs G"
+  assumes dom_parent_subset_vertices: "dom (parent s) \<subseteq> dVs G"
   assumes parent_edge: "\<lbrakk> v \<noteq> src; parent s v = Some u \<rbrakk> \<Longrightarrow> (u, v) \<in> G"
   assumes distance_parent:
     "\<lbrakk> v \<noteq> src; parent s v = Some u \<rbrakk> \<Longrightarrow> distance s v = Some m \<and> distance s u = Some n \<and> m = Suc n"
-  assumes distance_min: "distance s v = Some n \<Longrightarrow> shortest_dpath_length G src v = Some n"
+  assumes distance_min: "distance s v = Some n \<Longrightarrow> dist G src v = n"
 
-subsection \<open>\<close>
+  assumes in_queue_imp_discovered: "\<lbrakk> v \<noteq> src; v \<in> set (list (queue s)) \<rbrakk> \<Longrightarrow> discovered s v"
 
-lemma (in bfs) init_queue_subset_V:
+  assumes not_discovered_if_not_reachable: "\<not> reachable G src v \<Longrightarrow> \<not> discovered s v"
+
+  assumes "parent (parent s)"
+  assumes "discovered s v \<Longrightarrow> dpath_bet G (parent.follow (parent s) v) src v \<and> dpath_length (parent.follow (parent s) v) = dist G src v"
+
+subsection \<open>init\<close>
+
+lemma (in bfs) distance_src_init:
+  shows "distance init src = Some 0"
+  by (simp add: init_def)
+
+lemma (in bfs) parent_src_init:
+  shows "parent init src = None"
+  by (simp add: init_def)
+
+lemma (in bfs) invar_queue_init:
+  shows "invar (queue init)"
+  using invar_empty
+  by (auto simp add: init_def intro: invar_snoc)
+
+lemma (in bfs) queue_subset_vertices_init:
   shows "set (list (queue init)) \<subseteq> dVs G"
 proof -
   have "set (list (queue init)) = {src}"
     using invar_empty
     by (simp add: init_def list_snoc list_empty)
   also have "... \<subseteq> dVs G"
-    using src_in_V
+    using src_in_vertices
     by (simp add: dVs_def)
   finally show ?thesis
     .
 qed
 
-lemma (in bfs) init_distance_src:
-  shows "distance init src = Some 0"
+lemma (in bfs) dom_parent_subset_vertices_init:
+  shows "dom (parent init) \<subseteq> dVs G"
+  using src_in_vertices
   by (simp add: init_def)
 
-lemma (in bfs) init_parent_src:
-  shows "parent init src = Some src"
-  by (simp add: init_def)
-
-lemma (in bfs) init_parent_edge:
+lemma (in bfs) parent_edge_init:
   assumes "v \<noteq> src"
   assumes "parent init v = Some u"
   shows "(u, v) \<in> G"
   using assms
   by (simp add: init_def)
 
-lemma (in bfs) init_distance_parent:
+lemma (in bfs) distance_parent_init:
   assumes "v \<noteq> src"
   assumes "parent init v = Some u"
   shows "distance init v = Some m \<and> distance init u = Some n \<and> m = Suc n"
   using assms
   by (simp add: init_def)
 
-lemma (in bfs) init_distance_min:
-  shows "distance init v = Some n \<Longrightarrow> shortest_dpath_length G src v = Some n"
-  using src_in_V
-  by (simp add: init_def shortest_dpath_length_singleton split: if_splits)
+lemma (in bfs) distance_min_init:
+  assumes "distance init v = Some n"
+  shows "dist G src v = n"
+  sorry
 
-lemma (in bfs) init_bfs_invar:
+lemma (in bfs) in_queue_imp_discovered_init:
+  assumes "v \<noteq> src"
+  assumes "v \<in> set (list (queue init))"
+  shows "discovered v init"
+  using assms invar_empty
+  by (simp add: init_def list_snoc list_empty)
+
+lemma (in bfs) not_discovered_if_not_reachable_init:
+  assumes "\<not> reachable G src v"
+  shows "parent init v = None"
+  using assms
+  by (simp add: init_def)
+
+lemma (in bfs) bfs_invar_init:
   shows "bfs_invar empty is_empty head tail invar list src G snoc init"
   using
     bfs_axioms
-    init_queue_subset_V init_distance_src init_parent_src init_parent_edge init_distance_parent
-    init_distance_min
-  by (intro bfs_invar.intro bfs_invar_axioms.intro)
+    distance_src_init parent_src_init invar_queue_init queue_subset_vertices_init
+    dom_parent_subset_vertices_init parent_edge_init distance_parent_init distance_min_init
+    in_queue_imp_discovered_init not_discovered_if_not_reachable_init
+  by unfold_locales
 
 subsection \<open>\<close>
 
-section \<open>Termination\<close>
+subsubsection \<open>\<close>
 
-(* TODO *)
-lemma (in bfs) invar_queue:
-  shows "invar (queue s)"
-  sorry
-
-(* TODO *)
-lemma (in bfs) dom_parent_subset_V:
-  shows "dom (parent s) \<subseteq> dVs G"
-  sorry
-
-(* TODO *)
-lemma (in bfs) fold_insert:
-  assumes "finite A"
-  assumes "x \<notin> A"
-  shows "g (Finite_Set.fold f z (insert x A)) = g (f x (Finite_Set.fold f z A))"
-  sorry
-
-subsubsection \<open>parent\<close>
-
-lemma (in bfs) parent_discover_cong:
-  shows
-    "parent (discover u v s) =
-      parent s ++ (if discovered v s then Map.empty else [v \<mapsto> u])"
-  by (simp add: discover_def)
-
-lemma (in bfs) discovered_fold_cong:
-  assumes "finite N"
-  assumes "v \<notin> N"
-  shows "discovered v (Finite_Set.fold (discover u) s N) = discovered v s"
+lemma (in bfs) invar_queue_loop:
+  assumes "invar (queue s)"
+  assumes "dom (parent s) \<subseteq> dVs G"
+  shows "invar (queue (loop s))"
   using assms
-  by (induct N) (simp_all add: discovered_def fold_insert parent_discover_cong)
-
-lemma (in bfs) parent_fold_discover_insert:
-  assumes "finite N"
-  assumes "v \<notin> N"
-  shows
-    "parent (Finite_Set.fold (discover u) s (insert v N)) =
-      parent (Finite_Set.fold (discover u) s N) ++
-      (if discovered v s then Map.empty else [v \<mapsto> u])"
-  using assms
-  by (simp add: fold_insert parent_discover_cong discovered_fold_cong)
-
-lemma (in bfs) parent_fold_discover_cong:
-  assumes "finite N"
-  shows
-    "parent (Finite_Set.fold (discover u) s N) =
-      parent s ++ (\<lambda>v. if v \<in> N \<and> \<not> discovered v s then Some u else None)"
-  using assms
-  by (induct N) (auto simp add: parent_fold_discover_insert map_add_def)
-
-(*
-lemma (in bfs) parent_discover_comm:
-  shows
-    "parent \<circ> (discover u v) \<circ> (discover u w) =
-      parent \<circ> (discover u w) \<circ> (discover u v)"
-proof
-  fix s
-  show
-    "(parent \<circ> (discover u v) \<circ> (discover u w)) s =
-      (parent \<circ> (discover u w) \<circ> (discover u v)) s"
-  proof (cases "v = w")
+proof (induct rule: bfs_induct[OF assms])
+  case (1 s)
+  thus ?case
+  proof (cases "cond s")
     case True
-    thus ?thesis
-      by simp
+    hence loop:
+      "loop s =
+        loop (Finite_Set.fold (traverse_edge (head (queue s))) (s\<lparr>queue := tail (queue s)\<rparr>) (out_neighborhood G (head (queue s))))"
+      unfolding loop.psimps[OF "1.hyps"(1)]
+      by metis
+    show ?thesis
+      unfolding loop
+      using True "1.prems"
+      by (intro tbd "1.hyps"(2))
   next
     case False
-    fix s
-    have "dom [v \<mapsto> u] \<inter> dom [w \<mapsto> u] = {}"
-      using False
-      by simp
-    hence "[v \<mapsto> u] ++ [w \<mapsto> u] = [w \<mapsto> u] ++ [v \<mapsto> u]"
-      by (intro map_add_comm)
     thus ?thesis
-      using parent_discover_cong
-      by simp
+      using "1.hyps"(1) "1.prems"(1)
+      by (simp add: loop.psimps)
   qed
 qed
-*)
 
-subsubsection \<open>queue\<close>
+lemma (in bfs_invar) invar_queue_loop:
+  shows "invar (queue (loop s))"
+  using invar_queue dom_parent_subset_vertices
+  by (intro invar_queue_loop)
 
-lemma (in bfs) queue_discover_cong:
-  shows
-    "list (queue (discover u v s)) =
-      list (queue s) @ (if discovered v s then Nil else [v])"
-  using invar_queue[where ?s = s]
-  by (simp add: discover_def list_snoc)
+lemma (in bfs) invar_queue_bfs:
+  shows "invar (queue bfs)"
+  using bfs_invar_init
+  by (intro bfs_invar.invar_queue_loop)
 
-lemma (in bfs) queue_fold_discover_insert:
-  assumes "finite N"
-  assumes "v \<notin> N"
-  shows
-    "mset (list (queue (Finite_Set.fold (discover u) s (insert v N)))) =
-      mset (list (queue (Finite_Set.fold (discover u) s N))) +
-      (if discovered v s then {#} else {#v#})"
-  using assms
-  by (simp add: fold_insert queue_discover_cong discovered_fold_cong)
+subsubsection \<open>\<close>
 
-lemma (in bfs) queue_fold_discover_cong:
-  assumes "finite N"
-  shows
-    "mset (list (queue (Finite_Set.fold (discover u) s N))) =
-      mset (list (queue s)) + {#v \<in># mset_set N. \<not> discovered v s#}"
-  using assms
-  by (induct N) (simp_all add: queue_fold_discover_insert)
-
-lemma (in bfs) termination_aux:
-  assumes "S = {v \<in> (out_neighborhood G u). \<not> discovered v s}"
-  assumes
-    "dom (parent s ++
-      (\<lambda>v. if v \<in> (out_neighborhood G u) \<and> \<not> discovered v s then Some u else None)) =
-      dom (parent s) \<union> S"
-  shows
-    "card (dom (parent s ++
-      (\<lambda>v. if v \<in> (out_neighborhood G u) \<and> \<not> discovered v s then Some u else None))) =
-      card (dom (parent s)) + card S"
+lemma (in bfs)
+  assumes cond: "cond s"
+  assumes invar_queue: "invar (queue s)"
+  assumes "dom (parent s) \<subseteq> dVs G"
+  assumes "\<lbrakk> v \<noteq> src; v \<in> set (list (queue s)) \<rbrakk> \<Longrightarrow> discovered s v"
+  shows "\<lbrakk> v \<noteq> src; v \<in> set (list (queue (fold s))) \<rbrakk> \<Longrightarrow> discovered v (fold s)"
 proof -
-  have "finite (dom (parent s))"
-    using dom_parent_subset_V[where ?s = s] vertices_finite
-    by (auto intro: finite_subset)
-  moreover have "finite {v \<in> (out_neighborhood G u). \<not> discovered v s}"
-    using out_neighborhood_finite
+  have *: "invar (queue (s\<lparr>queue := tail (queue s)\<rparr>))"
+    using cond invar_queue invar_tail
+  by (simp add: is_empty cond_def)
+  assume
+    "v \<noteq> src"
+    "v \<in># mset (list (queue (local.fold s)))"
+  hence
+    "v \<in># mset (list (queue (s\<lparr>queue := tail (queue s)\<rparr>))) +
+      {#v \<in># mset_set (out_neighborhood G (head (queue s))). \<not> discovered v (s\<lparr>queue := tail (queue s)\<rparr>)#}"
+    unfolding mset_list_queue_fold_cong[OF * out_neighborhood_finite]
+    by blast
+  hence "v \<in> set (list (queue (s\<lparr>queue := tail (queue s)\<rparr>))) \<or>
+      v \<in> (out_neighborhood G (head (queue s))) \<and> \<not> discovered v (s\<lparr>queue := tail (queue s)\<rparr>)"
+    by (simp add: out_neighborhood_finite)
+    thm in_multiset_in_set
+    using * out_neighborhood_finite
+    sledgehammer
+    using mset_list_queue_fold_cong
+    try0
+    thm mset_list_queue_fold_cong[OF * out_neighborhood_finite]
+    apply (auto simp add: mset_list_queue_fold_cong)
+    sledgehammer
+    thm tbd
     by simp
-  moreover have "dom (parent s) \<inter> S = {}"
-    by (auto simp add: assms discovered_def)
-  ultimately show ?thesis
-    using assms
-    by (simp add: card_Un_disjoint)
+  show ?thesis
+    thm parent_fold_cong
+    thm mset_list_queue_fold_cong
+
+lemma (in bfs) in_queue_imp_discovered_loop:
+  assumes "invar (queue s)"
+  assumes "dom (parent s) \<subseteq> dVs G"
+  assumes "\<lbrakk> v \<noteq> src; v \<in> set (list (queue s)) \<rbrakk> \<Longrightarrow> discovered s v"
+  shows "\<lbrakk> v \<noteq> src; v \<in> set (list (queue (loop s))) \<rbrakk> \<Longrightarrow> discovered v (loop s)"
+  using assms
+proof (induct rule: bfs_induct[OF assms(1, 2)])
+  case (1 s)
+  thus ?case
+  proof (cases "cond s")
+    case True
+    hence loop:
+      "loop s =
+        loop (Finite_Set.fold (traverse_edge (head (queue s))) (s\<lparr>queue := tail (queue s)\<rparr>) (out_neighborhood G (head (queue s))))"
+      unfolding loop.psimps[OF "1.hyps"(1)]
+      by metis
+
+    have *: "v \<in> set (list (queue
+                 (loop
+                   (Finite_Set.fold (traverse_edge (head (queue s)))
+                     (s\<lparr>queue := tail (queue s)\<rparr>)
+                     (out_neighborhood G (head (queue s)))))))"
+      using "1.prems"(2)
+      by (simp add: loop)
+
+    have **: "invar
+ (queue
+   (Finite_Set.fold (traverse_edge (head (queue s))) (s\<lparr>queue := tail (queue s)\<rparr>)
+     (out_neighborhood G (head (queue s)))))"
+      using True "1.prems"(3, 4)
+      apply (intro tbd(1)) by (simp add: loop)+
+
+    have ***: "dom (state.parent
+      (Finite_Set.fold (traverse_edge (head (queue s))) (s\<lparr>queue := tail (queue s)\<rparr>)
+        (out_neighborhood G (head (queue s)))))
+\<subseteq> dVs G"
+      using True "1.prems"(3, 4)
+      apply (intro tbd(2)) by (simp add: loop)+
+
+    have "(v \<noteq> src \<Longrightarrow>
+ v \<in> set (list (queue
+                  (Finite_Set.fold (traverse_edge (head (queue s)))
+                    (s\<lparr>queue := tail (queue s)\<rparr>)
+                    (out_neighborhood G (head (queue s)))))) \<Longrightarrow>
+ discovered v
+  (Finite_Set.fold (traverse_edge (head (queue s))) (s\<lparr>queue := tail (queue s)\<rparr>)
+    (out_neighborhood G (head (queue s)))))"
+      thm "1.prems"
+      find_theorems name: fold_cong
+      sledgehammer
+
+    show ?thesis
+      using "1.hyps"(2)[OF True "1.prems"(1)]
+      unfolding loop
+      using "1.prems"(3)
+      using True "1.prems"
+      apply (auto simp add: loop intro: tbd "1.hyps"(2))
+      thm "1.prems"
+      thm "1.hyps"(2)
+      thm "1.hyps"(2)[OF True "1.prems"(1) * ** ***]
+      unfolding loop
+      using True "1.prems"(1, 2, 3)
+      apply (intro tbd "1.hyps"(2))
+      apply (auto simp add: loop)
+      using True "1.prems"(1, 2, 3)
+      apply (intro "1.hyps"(2))
+           apply auto
+      apply (simp add: loop)
+        apply (simp add: cond_def invar_queue_fold invar_tail is_empty out_neighborhood_finite)
+      sledgehammer
+      sledgehammer
+      thm "1.prems"
+      thm "1.hyps"
+      sorry
+  next
+    case False
+    thus ?thesis
+      using "1.hyps"(1) "1.prems"(1, 2, 5)
+      by (simp add: loop.psimps)
+  qed
 qed
 
-lemma (in bfs) termination_aux2:
-  fixes s :: "('q, 'v) state"
-  assumes "cond s"
-  shows
-    "card (dVs G) +
-      length (list (queue (s\<lparr>queue := (tail (queue s))\<rparr>))) -
-      card (dom (parent (s\<lparr>queue := (tail (queue s))\<rparr>))) <
-      card (dVs G) +
-      length (list (queue s)) -
-      card (dom (parent s))"
-proof -
-  have "list (queue s) \<noteq> Nil"
-    using invar_queue[where ?s = s] assms
-    by (simp add: is_empty cond_def)
-  hence "length (list (queue (s\<lparr>queue := (tail (queue s))\<rparr>))) < length (list (queue s))"
-    using invar_queue[where ?s = s]
-    by (simp add: length_tail)
-  moreover have "card (dom (parent s)) \<le> card (dVs G)"
-    using vertices_finite dom_parent_subset_V
-    by (intro card_mono)
-  ultimately show ?thesis
+lemma (in bfs_invar) in_queue_imp_discovered_loop:
+  assumes "v \<noteq> src"
+  assumes "v \<in> set (list (queue (loop s)))"
+  shows "discovered v (loop s)"
+  using invar_queue dom_parent_subset_vertices in_queue_imp_discovered assms
+  by (intro in_queue_imp_discovered_loop)
+
+lemma (in bfs) in_queue_imp_discovered_bfs:
+  assumes "v \<noteq> src"
+  assumes "v \<in> set (list (queue bfs))"
+  shows "discovered v bfs"
+  using bfs_invar_init assms
+  by (intro bfs_invar.in_queue_imp_discovered_loop)
+
+subsubsection \<open>\<close>
+(**)
+
+lemma (in bfs) discovered_imp_reachable_fold:
+  assumes "invar (queue s)"
+  assumes "dom (parent s) \<subseteq> dVs G"
+  assumes IH: "\<And>v. discovered s v \<Longrightarrow> reachable G src v"
+  shows "discovered v (fold s) \<Longrightarrow> reachable G src v"
+proof (rule ccontr)
+  fix v
+  assume discovered: "discovered v (fold s)"
+  assume not_reachable: "\<not> reachable G src v"
+
+  let ?u = "head (queue s)"
+  let ?q = "tail (queue s)"
+
+  have "v \<in> dom (parent (fold s))"
+    using discovered
+    by (simp add: discovered_def)
+  hence "v \<in> dom (\<lambda>v. if v \<in> (out_neighborhood G ?u) \<and> \<not> discovered v (s\<lparr>queue := ?q\<rparr>) then Some ?u else None)"
+    using out_neighborhood_finite not_reachable IH
+    by (auto simp add: parent_fold_cong discovered_def)
+  hence in_neighborhood: "v \<in> (out_neighborhood G ?u)"
+    unfolding domIff
+    by meson
+
+  (*
+    TODO: add invariant
+      v \<in># mset (list (queue s)) \<Longrightarrow> discovered s v
+      or
+      v \<in> ran (parent (fold s)) \<Longrightarrow> v \<in> dom (parent s)
+  *)
+  have "discovered ?u s"
+    sorry
+  hence "reachable G src ?u"
+    thm IH
+    by (intro IH)
+  hence "reachable G src v"
+    using in_neighborhood
+    by (auto simp add: out_neighborhood_def intro: reachable_trans)
+  thus "False"
+    using not_reachable
     by simp
 qed
 
-termination (in bfs) loop
-proof (relation "measure (\<lambda>s. card (dVs G) + length (list (queue s)) - card (dom (parent s)))")
-  fix s u q
-  assume assms:
-    "cond s"
-    "u = head (queue s)"
-    "q = tail (queue s)"
-  
-  define S :: "'v set" where "S \<equiv> {v \<in> (out_neighborhood G u). \<not> discovered v (s\<lparr>queue := q\<rparr>)}"
-  
-  have
-    "dom (\<lambda>v. if v \<in> (out_neighborhood G u) \<and> \<not> discovered v (s\<lparr>queue := q\<rparr>) then Some u else None) =
-      {v \<in> (out_neighborhood G u). \<not> discovered v (s\<lparr>queue := q\<rparr>)}"
-    by (simp add: dom_def)
-  hence
-    "dom (parent (s\<lparr>queue := q\<rparr>) ++
-      (\<lambda>v. if v \<in> (out_neighborhood G u) \<and> \<not> discovered v (s\<lparr>queue := q\<rparr>) then Some u else None)) =
-      dom (parent (s\<lparr>queue := q\<rparr>)) \<union> S"
-    by (auto simp add: S_def)
-  with S_def have
-    "card (dom (parent (s\<lparr>queue := q\<rparr>) ++
-      (\<lambda>v. if v \<in> (out_neighborhood G u) \<and> \<not> discovered v (s\<lparr>queue := q\<rparr>) then Some u else None))) =
-      card (dom (parent (s\<lparr>queue := q\<rparr>))) + card S"
-    by (intro termination_aux) blast+
-  hence
-    "card (dom (parent (Finite_Set.fold (discover u) (s\<lparr>queue := q\<rparr>) (out_neighborhood G u)))) =
-      card (dom (parent (s\<lparr>queue := q\<rparr>))) + card S"
-    using out_neighborhood_finite
-    by (simp add: parent_fold_discover_cong)
-  moreover have
-    "length (list (queue (Finite_Set.fold (discover u) (s\<lparr>queue := q\<rparr>) (out_neighborhood G u)))) =
-      length (list (queue (s\<lparr>queue := q\<rparr>))) + card S"
-    unfolding size_mset[symmetric]
-    using out_neighborhood_finite
-    by (simp add: S_def queue_fold_discover_cong)
-  ultimately have
-    "card (dVs G) +
-      length (list (queue (Finite_Set.fold (discover u) (s\<lparr>queue := q\<rparr>) (out_neighborhood G u)))) -
-      card (dom (parent (Finite_Set.fold (discover u) (s\<lparr>queue := q\<rparr>) (out_neighborhood G u)))) =
-      card (dVs G) +
-      length (list (queue (s\<lparr>queue := q\<rparr>))) + card (out_neighborhood G u - dom (parent (s\<lparr>queue := q\<rparr>))) -
-      (card (dom (parent (s\<lparr>queue := q\<rparr>))) + card (out_neighborhood G u - dom (parent (s\<lparr>queue := q\<rparr>))))"
-    by simp
-  also have "... = card (dVs G) + length (list (queue (s\<lparr>queue := q\<rparr>))) - card (dom (parent (s\<lparr>queue := q\<rparr>)))"
-    by simp
-  also have "... < card (dVs G) + length (list (queue s)) - card (dom (parent s))"
-    unfolding assms(3)
-    using assms(1)
-    by (intro termination_aux2)
-  finally show
-    "Finite_Set.fold (discover u) (s\<lparr>queue := q\<rparr>) (out_neighborhood G u)
-      \<rightarrow>\<^bsub>measure (\<lambda>s. card (dVs G) + length (list (queue s)) - card (dom (parent s)))\<^esub>s"
-    by simp
-qed simp
+lemma (in bfs) discovered_imp_reachable_loop:
+  assumes "invar (queue s)"
+  assumes "dom (parent s) \<subseteq> dVs G"
+  assumes "\<And>v. discovered s v \<Longrightarrow> reachable G src v"
+  shows "discovered v (loop s) \<Longrightarrow> reachable G src v"
+  using assms
+proof (induct rule: bfs_induct[OF assms(1, 2)])
+  case (1 s)
+  thus ?case
+  proof (cases "cond s")
+    case True
+    hence loop: "loop s = loop (fold s)"
+      unfolding loop.psimps[OF "1.hyps"(1)]
+      by metis
+
+    show ?thesis
+    proof (intro "1.hyps"(2))
+      show "\<And>v. discovered v (local.fold s) \<Longrightarrow> src \<rightarrow>\<^sup>*\<^bsub>G\<^esub> v"
+        using "1.prems"(2-)
+        by (rule discovered_imp_reachable_fold)
+    qed using "1.prems" apply (auto intro: tbd)
+      using True "1.prems"
+      unfolding loop
+      apply (rule "1.hyps"(2))
+      sledgehammer
+      thm "1.hyps"(2)
+      
+      thm discovered_imp_reachable_fold
+      thm "1.hyps"(2)[OF _ _ _ _ discovered_imp_reachable_fold]
+      by (smt "1.hyps"(2) bfs.tbd(1) bfs.tbd(2) bfs_axioms discovered_imp_reachable_fold surjective update_convs(1))
+    thm discovered_imp_reachable_fold
+    find_theorems "\<And>_. _"
+find_theorems name: allI
+      by (intr tbd discovered_imp_reachable_fold "1.hyps"(2))
+  next
+    case False
+    thus ?thesis
+      using "1.hyps"(1) "1.prems"(1, 4)
+      by (simp add: loop.psimps)
+  qed
+qed
+
+lemma (in bfs_invar) discovered_imp_reachable_loop:
+  assumes "discovered v (loop s)"
+  shows "reachable G src v"
+  using invar_queue dom_parent_subset_vertices not_discovered_if_not_reachable assms
+  by (intro discovered_imp_reachable_loop)
+
+lemma (in bfs) not_discovered_if_not_reachable_bsf:
+  assumes "discovered v bfs"
+  shows "reachable G src v"
+  using bfs_invar_init assms
+  by (intro bfs_invar.discovered_imp_reachable_loop)
 
 section \<open>Correctness\<close>
 
