Graph_Theory/Dpath.thy
@@ -2,11 +2,90 @@ theory Dpath
   imports
     Dgraph
     Ports.Berge_to_DDFS
+    Ports.Mitja_to_DDFS
+    Ports.Noschinski_to_DDFS
 begin
 
-type_synonym 'v dpath = "'v list"
+type_synonym 'a dpath = "'a list"
 
-abbreviation dpath_length :: "'v dpath \<Rightarrow> nat" where
+lemmas dpath_induct = edges_of_dpath.induct
+
+lemma dpath_rev_induct:
+  assumes "P []"
+  assumes "\<And>v. P [v]"
+  assumes "\<And>u v l. P (l @ [u]) \<Longrightarrow> P (l @ [u, v])"
+  shows "P p"
+  using assms
+proof (induct "rev p" arbitrary: p rule: dpath_induct)
+  case 1
+  thus ?case
+    by simp
+next
+  case (2 _)
+  thus ?case
+    by simp
+next
+  case (3 v v' l)
+  have "rev l @ [v'] @ [v] = p"
+    using "3.hyps"(2)
+    unfolding append.assoc[symmetric] rev.simps(2)[symmetric]
+    by auto
+  hence "rev l @ [v', v] = p"
+    by simp
+  moreover have "P (rev l @ [v', v])"
+    using 3
+    by simp
+  ultimately show ?case
+    by simp
+qed
+
+text \<open>The length of a @{term dpath} is the number of its edges.\<close>
+
+abbreviation dpath_length :: "'a dpath \<Rightarrow> nat" where
   "dpath_length p \<equiv> length (edges_of_dpath p)"
+
+
+lemma dpath_length_Cons:
+  assumes "vs \<noteq> []"
+  shows "dpath_length (v # vs) = dpath_length vs + 1"
+  apply (subst hd_Cons_tl[OF assms, symmetric])
+  apply (subst edges_of_dpath.simps(3))
+  apply (subst list.size(4))
+  apply (subst hd_Cons_tl[OF assms])
+  apply (subst One_nat_def)
+  ..
+
+lemma dpath_length_snoc:
+  assumes "vs \<noteq> []"
+  shows "dpath_length (vs @ [v]) = dpath_length vs + 1"
+  using assms
+  by (simp add: edges_of_dpath_append_3)
+
+lemma dpath_length_append:
+  assumes "p \<noteq> []"
+  shows "dpath_length (p @ q) = dpath_length p + dpath_length (last p # q)"
+  using assms
+  by (simp add: edges_of_dpath_append_3)
+
+lemma dpath_length_append_2:
+  assumes "p \<noteq> []"
+  assumes "q \<noteq> []"
+  assumes "last p = hd q"
+  shows "dpath_length (p @ tl q) = dpath_length p + dpath_length q"
+  using assms
+  by (simp add: dpath_length_append)
+
+section \<open>Reachability\<close>
+
+lemma reachable_iff_dpath_bet:
+  shows "reachable G u v \<longleftrightarrow> (\<exists>p. dpath_bet G p u v)"
+  by (auto simp add: reachable_awalk intro: awalk_imp_dpath dpath_imp_awalk)
+
+lemma reachable_trans:
+  assumes "reachable G u v"
+  assumes "reachable G v w"
+  shows "reachable G u w"
+  using assms
+  by (blast intro: trancl_trans)
 
 end
