Tbd.thy
@@ -1,11 +1,112 @@
 theory Tbd
-  imports "HOL-Data_Structures.Set_Specs"
+  imports Main
 begin
 
-(* locale tbd = Set where insert = insert for insert :: "'a \<Rightarrow> 's \<Rightarrow> 's" (* for typing purposes only *) +
-  fixes fold :: "('a \<Rightarrow> 'b \<Rightarrow> 'b) \<Rightarrow> 's \<Rightarrow> 'b \<Rightarrow> 'b" *)
+(* TODO *)
+definition follow_invar :: "('a \<rightharpoonup> 'a) \<Rightarrow> bool" where
+  "follow_invar parent \<equiv>
+    (\<forall>v. \<exists>u. (u = v \<or> (u, v) \<in> {(u, v) |u v. parent v = Some u}\<^sup>+) \<and> parent u = None) \<and>
+    (\<forall>u v. parent v = Some u \<longrightarrow> v \<noteq> u) \<and> 
+    finite {(u, v) |u v. parent v = Some u}"
 
-locale tbd =
-  fixes fold :: "('a \<Rightarrow> 'b \<Rightarrow> 'b) \<Rightarrow> 'a set \<Rightarrow> 'b \<Rightarrow> 'b"
+(* TODO *)
+definition follow_invar' :: "('a \<rightharpoonup> 'a) \<Rightarrow> bool" where
+  "follow_invar' parent \<equiv> wf {(u, v) |u v. parent v = Some u}"
+
+locale parent = 
+  fixes parent :: "'a \<rightharpoonup> 'a"
+  (* fixes parent_rel :: "'a \<Rightarrow> 'a \<Rightarrow> bool" *)
+  assumes follow_invar': "follow_invar' parent"
+
+function (in parent) (domintros) follow :: "'a \<Rightarrow> 'a list" where
+  "follow v = (case parent v of None \<Rightarrow> [v] | Some u \<Rightarrow> v # follow u)"
+  by pat_completeness auto
+
+section \<open>Termination\<close>
+
+lemma (in parent)
+  assumes "parent v = None"
+  shows "follow_dom v"
+  using assms
+  by (auto intro: follow.domintros)
+
+lemma (in parent)
+  assumes "parent v = Some u"
+  assumes "follow_dom u"
+  shows "Wellfounded.accp follow_rel v"
+  using assms
+  by (auto intro: follow.domintros)
+
+lemma (in parent) follow_dom_if_follow_rel_wfP:
+  assumes "wfP follow_rel"
+  shows "follow_dom v"
+  using assms
+  by (intro accp_wfPD)
+
+lemma (in parent) follow_dom_if_follow_rel_wf:
+  assumes "wf {(u, v) |u v. follow_rel u v}"
+  shows "follow_dom v"
+  using assms
+  by (intro follow_dom_if_follow_rel_wfP) (simp add: wfP_def)
+
+lemma (in parent) follow_rel_eq_parent:
+  shows "follow_rel = (\<lambda>u v. parent v = Some u)"
+  by (fastforce simp add: follow_rel.simps)
+
+lemma (in parent) follow_rel_wf:
+  shows "wf {(u, v) |u v. follow_rel u v}"
+  using follow_invar'
+  by (simp add: follow_invar'_def follow_rel_eq_parent)
+
+lemma (in parent) follow_dom:
+  shows "follow_dom v"
+  using follow_rel_wf
+  by (intro follow_dom_if_follow_rel_wf)
+
+section \<open>\<close>
+
+lemma (in parent) follow_psimps:
+  shows "follow v = (case parent v of None \<Rightarrow> [v] | Some u \<Rightarrow> v # follow u)"
+  using follow_dom
+  by (intro follow.psimps)
+
+lemma (in parent) follow_non_empty:
+  shows "follow v \<noteq> []"
+  by (simp add: follow_psimps split: option.split)
+
+lemma (in parent) follow_ConsD:
+  assumes "follow u = v # p"
+  shows "v = u"
+  using assms
+  by (simp add: follow_psimps split: option.splits(2))
+
+lemma (in parent) follow_Cons_ConsD:
+  assumes "follow v = v # u # p"
+  shows
+    "follow u = u # p"
+    "parent v = Some u"
+  using assms
+  by (auto simp add: follow_psimps split: option.splits(2))
+
+lemma (in parent) follow_Cons_ConsE:
+  assumes "follow v = v # p"
+  assumes "p \<noteq> Nil"
+  obtains u where "follow u = p"
+  using assms
+  by (simp add: follow_psimps split: option.splits(2))
+
+lemma (in parent) follow_appendD:
+  assumes "follow v = p @ u # p'"
+  shows "follow u = u # p'"
+  using assms
+  by (induct p arbitrary: v) (auto dest: follow_ConsD elim: follow_Cons_ConsE)
+
+(* TODO *)
+lemma (in parent) tbd:
+  assumes "follow v1 = p1 @ u # p1'"
+  assumes "follow v2 = p2 @ u # p2'"
+  shows "p1' = p2'"
+  using follow_appendD[OF assms(1)] follow_appendD[OF assms(2)]
+  by simp
 
 end
