Misc.thy
@@ -5,11 +5,4 @@ begin
 
 section \<open>Queues\<close>
 
-lemma (in Queue) length_tail:
-  assumes "invar q"
-  assumes "list q \<noteq> Nil"
-  shows "length (list (tail q)) = length (list q) - 1"
-  using assms list_head
-  by (simp add: list_tail)
-
 end
